main.ml
@@ -7,15 +7,7 @@ let nat_of_int n = nat_of_integer (Z.of_int n)
 
 let str_of_nat n = Z.to_string (integer_of_nat n)
 
-let str_of_compare = function
-  | LT -> "LT"
-  | GT -> "GT"
-  | EQ -> "EQ"
-
-let compare_height_set x y = match x, y with
-  | RBT_set x, RBT_set y -> compare_height_rbt x y
-
-let rec run i l = nat_set_upt (nat_of_int (i * l)) (nat_of_int ((i + 1) * l))
+let rec run i l = nat_upt (nat_of_int (i * l)) (nat_of_int ((i + 1) * l))
 
 let gen size =
   let rec loop acc = function
@@ -30,7 +22,6 @@ let rec union n l =
   (* let cur = nat_set (List.map nat_of_int (gen l)) in *)
   if n = 0 then cur else
     let rest = union (n - 1) l in
-    (* let _ = Printf.printf "%d %d %s\n" l (n * l) (str_of_compare (compare_height_set cur rest)) in *)
     un_nat_set cur rest
 
 let _ = union n l
