RBT_height.thy
@@ -2,9 +2,6 @@ theory RBT_height
   imports "HOL-Library.Code_Target_Nat" "Containers.Containers" RBT_set_opt
 begin
 
-(* We define a type of sorted and distinct lists from which we can create an RBT more efficiently
-   than using the built-in function for converting lists into sets. *)
-
 typedef (overloaded) 'a sdlist = "{xs :: ('a :: ccompare) list.
   case ID CCOMPARE('a) of None \<Rightarrow> xs = []
   | Some c \<Rightarrow> linorder.sorted (le_of_comp c) xs \<and> distinct xs}"
@@ -13,7 +10,7 @@ typedef (overloaded) 'a sdlist = "{xs :: ('a :: ccompare) list.
 
 setup_lifting type_definition_sdlist
 
-lemma sset_rbt:
+lemma is_rbt_rbtreeify:
   fixes xs :: "('a :: ccompare) list"
     and c :: "'a comparator"
   assumes assms: "ID ccompare = Some c" "linorder.sorted (le_of_comp c) xs" "distinct xs"
@@ -21,9 +18,9 @@ lemma sset_rbt:
   using assms linorder.is_rbt_rbtreeify[OF ID_ccompare[OF assms(1)], of "map (\<lambda>x. (x, ())) xs"]
   by (auto simp: comp_def)
 
-lift_definition sset :: "('a :: ccompare) sdlist \<Rightarrow> 'a set_rbt" is
+lift_definition rbt_of_sdlist :: "('a :: ccompare) sdlist \<Rightarrow> 'a set_rbt" is
   "\<lambda>xs. rbtreeify (map (\<lambda>x. (x, ())) xs)"
-  using sset_rbt
+  using is_rbt_rbtreeify
   by fastforce
 
 lemma rbt_comp_lookup_iff_in_set:
@@ -37,9 +34,9 @@ lemma rbt_comp_lookup_iff_in_set:
   by (auto simp: rbt_comp_lookup[OF ID_ccompare'[OF assms(1)]] assms(1) map_of_map_Pair_const
       comp_def)
 
-lemma RBT_set_sset:
+lemma RBT_set_rbt_of_sdlist:
   fixes xs :: "('a :: ccompare) sdlist"
-  shows "RBT_set (sset xs) = set (Rep_sdlist xs)"
+  shows "RBT_set (rbt_of_sdlist xs) = set (Rep_sdlist xs)"
   unfolding RBT_set_def
   apply transfer
   using rbt_comp_lookup_iff_in_set
@@ -60,7 +57,7 @@ lemma distinct_remdups_adj: "sorted xs \<Longrightarrow> distinct (remdups_adj x
 end
 
 lift_definition sdlist_of_list :: "('a :: ccompare) list \<Rightarrow> 'a sdlist" is
-  "\<lambda>xs :: 'a list. case ID CCOMPARE('a) of None \<Rightarrow> []
+  "\<lambda>xs. case ID CCOMPARE('a) of None \<Rightarrow> []
   | Some c \<Rightarrow> remdups_adj (ord.quicksort (lt_of_comp c) xs)"
   using linorder.sorted_remdups_adj[OF ID_ccompare linorder.sorted_sort[OF ID_ccompare]]
   using linorder.distinct_remdups_adj[OF ID_ccompare linorder.sorted_sort[OF ID_ccompare]]
@@ -77,39 +74,33 @@ lemma set_sdlist_of_list:
   using linorder.set_sort[OF ID_ccompare] quicksort_conv_sort_key
   by fastforce
 
-lemma set_code:
-  fixes xs :: "('a :: ccompare) list"
-  shows "set xs = (case ID CCOMPARE('a) of None \<Rightarrow> Code.abort (STR ''set: ccompare = None'')
-    (\<lambda>_. set xs)
-  | Some _ \<Rightarrow> RBT_set (sset (sdlist_of_list xs)))"
-  by (auto simp: RBT_set_sset set_sdlist_of_list split: option.splits)
+definition sset :: "'a list \<Rightarrow> 'a set" where
+  "sset = set"
 
-definition nat_set_upt :: "nat \<Rightarrow> nat \<Rightarrow> nat list" where
-  "nat_set_upt i j = [i..<j]"
+lemma sset_code[code]:
+  fixes xs :: "('a :: ccompare) list"
+  shows "sset xs = (case ID CCOMPARE('a) of None \<Rightarrow> Code.abort (STR ''sset: ccompare = None'')
+    (\<lambda>_. sset xs)
+  | Some _ \<Rightarrow> RBT_set (rbt_of_sdlist (sdlist_of_list xs)))"
+  by (auto simp: sset_def RBT_set_rbt_of_sdlist set_sdlist_of_list split: option.splits)
+
+definition nat_upt :: "nat \<Rightarrow> nat \<Rightarrow> nat list" where
+  "nat_upt i j = [i..<j]"
 
 definition nat_set :: "nat list \<Rightarrow> nat set" where
   "nat_set = set"
 
+definition nat_sset :: "nat list \<Rightarrow> nat set" where
+  "nat_sset = sset"
+
 definition un_nat_set :: "nat set \<Rightarrow> nat set \<Rightarrow> nat set" where
   "un_nat_set X Y = X \<union> Y"
 
-definition int_nat_set :: "nat set \<Rightarrow> nat set \<Rightarrow> nat set" where
-  "int_nat_set X Y = X \<inter> Y"
+definition inter_nat_set :: "nat set \<Rightarrow> nat set \<Rightarrow> nat set" where
+  "inter_nat_set X Y = X \<inter> Y"
 
-definition compare_height_rbt :: "(nat, unit) mapping_rbt \<Rightarrow> (nat, unit) mapping_rbt \<Rightarrow>
-  RBT_Impl.compare" where
-  "compare_height_rbt t1 t2 =
-    RBT_Impl.compare_height (RBT_Mapping2.impl_of t1) (RBT_Mapping2.impl_of t1)
-    (RBT_Mapping2.impl_of t2) (RBT_Mapping2.impl_of t2)"
-
-export_code nat_set_upt nat_set un_nat_set int_nat_set
-  nat_of_integer integer_of_nat compare_height_rbt RBT_set RBT_Impl.EQ
+export_code nat_upt nat_set nat_sset un_nat_set inter_nat_set nat_of_integer integer_of_nat
   in OCaml module_name RBT_height file_prefix "RBT_height_old"
-
-(*
-declare Set_Impl.set_code[code del]
-declare set_code[code]
-*)
 
 declare Set_union_code(1)[code del]
 declare rbt_union_code[code]
@@ -120,8 +111,7 @@ declare rbt_inter_code[code]
 declare Set_minus_code[code del]
 declare rbt_minus_code[code]
 
-export_code nat_set_upt nat_set un_nat_set int_nat_set
-  nat_of_integer integer_of_nat compare_height_rbt RBT_set RBT_Impl.EQ
+export_code nat_upt nat_set nat_sset un_nat_set inter_nat_set nat_of_integer integer_of_nat
   in OCaml module_name RBT_height file_prefix "RBT_height_opt"
 
 end
