RBT_set_opt.thy
@@ -2,77 +2,77 @@ theory RBT_set_opt
   imports "HOL-Library.RBT_Impl" "Containers.Set_Impl"
 begin
 
-type_synonym 'a urbt = "('a, unit) RBT_Impl.rbt"
-
-definition is_empty :: "'a urbt \<Rightarrow> bool" where
+definition is_empty :: "('a, 'b) rbt \<Rightarrow> bool" where
   "is_empty t \<longleftrightarrow> (case t of RBT_Impl.Empty \<Rightarrow> True | _ \<Rightarrow> False)"
 
 lemma is_empty_prop[simp]: "is_empty t \<longleftrightarrow> t = RBT_Impl.Empty"
   by (auto simp: is_empty_def split: RBT_Impl.rbt.splits)
 
-definition small_rbt :: "'a urbt \<Rightarrow> bool" where
+definition small_rbt :: "('a, 'b) rbt \<Rightarrow> bool" where
   "small_rbt t \<longleftrightarrow> bheight t < 6"
 
-definition flip_rbt :: "'a urbt \<Rightarrow> 'a urbt \<Rightarrow> bool" where
+definition flip_rbt :: "('a, 'b) rbt \<Rightarrow> ('a, 'b) rbt \<Rightarrow> bool" where
   "flip_rbt t1 t2 \<longleftrightarrow> bheight t2 < bheight t1"
 
-abbreviation MR where "MR l a r \<equiv> Branch RBT_Impl.R l a () r"
-abbreviation MB where "MB l a r \<equiv> Branch RBT_Impl.B l a () r"
+abbreviation MR where "MR l a b r \<equiv> Branch RBT_Impl.R l a b r"
+abbreviation MB where "MB l a b r \<equiv> Branch RBT_Impl.B l a b r"
 
-fun baliL :: "'a urbt \<Rightarrow> 'a \<Rightarrow> 'a urbt \<Rightarrow> 'a urbt" where
-  "baliL (MR (MR t1 a t2) b t3) c t4 = MR (MB t1 a t2) b (MB t3 c t4)"
-| "baliL (MR t1 a (MR t2 b t3)) c t4 = MR (MB t1 a t2) b (MB t3 c t4)"
-| "baliL t1 a t2 = MB t1 a t2"
+fun baliL :: "('a, 'b) rbt \<Rightarrow> 'a \<Rightarrow> 'b \<Rightarrow> ('a, 'b) rbt \<Rightarrow> ('a, 'b) rbt" where
+  "baliL (MR (MR t1 a b t2) a' b' t3) a'' b'' t4 = MR (MB t1 a b t2) a' b' (MB t3 a'' b'' t4)"
+| "baliL (MR t1 a b (MR t2 a' b' t3)) a'' b'' t4 = MR (MB t1 a b t2) a' b' (MB t3 a'' b'' t4)"
+| "baliL t1 a b t2 = MB t1 a b t2"
 
-fun baliR :: "'a urbt \<Rightarrow> 'a \<Rightarrow> 'a urbt \<Rightarrow> 'a urbt" where
-  "baliR t1 a (MR t2 b (MR t3 c t4)) = MR (MB t1 a t2) b (MB t3 c t4)"
-| "baliR t1 a (MR (MR t2 b t3) c t4) = MR (MB t1 a t2) b (MB t3 c t4)"
-| "baliR t1 a t2 = MB t1 a t2"
+fun baliR :: "('a, 'b) rbt \<Rightarrow> 'a \<Rightarrow> 'b \<Rightarrow> ('a, 'b) rbt \<Rightarrow> ('a, 'b) rbt" where
+  "baliR t1 a b (MR t2 a' b' (MR t3 a'' b'' t4)) = MR (MB t1 a b t2) a' b' (MB t3 a'' b'' t4)"
+| "baliR t1 a b (MR (MR t2 a' b' t3) a'' b'' t4) = MR (MB t1 a b t2) a' b' (MB t3 a'' b'' t4)"
+| "baliR t1 a b t2 = MB t1 a b t2"
 
-fun paint :: "color \<Rightarrow> 'a urbt \<Rightarrow> 'a urbt" where
+fun paint :: "color \<Rightarrow> ('a, 'b) rbt \<Rightarrow> ('a, 'b) rbt" where
   "paint c RBT_Impl.Empty = RBT_Impl.Empty"
-| "paint c (RBT_Impl.Branch _ l a () r) = RBT_Impl.Branch c l a () r"
+| "paint c (RBT_Impl.Branch _ l a b r) = RBT_Impl.Branch c l a b r"
 
-fun baldL :: "'a urbt \<Rightarrow> 'a \<Rightarrow> 'a urbt \<Rightarrow> 'a urbt" where
-  "baldL (MR t1 a t2) b t3 = MR (MB t1 a t2) b t3"
-| "baldL t1 a (MB t2 b t3) = baliR t1 a (MR t2 b t3)"
-| "baldL t1 a (MR (MB t2 b t3) c t4) = MR (MB t1 a t2) b (baliR t3 c (paint RBT_Impl.R t4))"
-| "baldL t1 a t2 = MR t1 a t2"
+fun baldL :: "('a, 'b) rbt \<Rightarrow> 'a \<Rightarrow> 'b \<Rightarrow> ('a, 'b) rbt \<Rightarrow> ('a, 'b) rbt" where
+  "baldL (MR t1 a b t2) a' b' t3 = MR (MB t1 a b t2) a' b' t3"
+| "baldL t1 a b (MB t2 a' b' t3) = baliR t1 a b (MR t2 a' b' t3)"
+| "baldL t1 a b (MR (MB t2 a' b' t3) a'' b'' t4) =
+  MR (MB t1 a b t2) a' b' (baliR t3 a'' b'' (paint RBT_Impl.R t4))"
+| "baldL t1 a b t2 = MR t1 a b t2"
 
-fun baldR :: "'a urbt \<Rightarrow> 'a \<Rightarrow> 'a urbt \<Rightarrow> 'a urbt" where
-  "baldR t1 a (MR t2 b t3) = MR t1 a (MB t2 b t3)"
-| "baldR (MB t1 a t2) b t3 = baliL (MR t1 a t2) b t3"
-| "baldR (MR t1 a (MB t2 b t3)) c t4 = MR (baliL (paint RBT_Impl.R t1) a t2) b (MB t3 c t4)"
-| "baldR t1 a t2 = MR t1 a t2"
+fun baldR :: "('a, 'b) rbt \<Rightarrow> 'a \<Rightarrow> 'b \<Rightarrow> ('a, 'b) rbt \<Rightarrow> ('a, 'b) rbt" where
+  "baldR t1 a b (MR t2 a' b' t3) = MR t1 a b (MB t2 a' b' t3)"
+| "baldR (MB t1 a b t2) a' b' t3 = baliL (MR t1 a b t2) a' b' t3"
+| "baldR (MR t1 a b (MB t2 a' b' t3)) a'' b'' t4 =
+  MR (baliL (paint RBT_Impl.R t1) a b t2) a' b' (MB t3 a'' b'' t4)"
+| "baldR t1 a b t2 = MR t1 a b t2"
 
-fun app :: "'a urbt \<Rightarrow> 'a urbt \<Rightarrow> 'a urbt" where
+fun app :: "('a, 'b) rbt \<Rightarrow> ('a, 'b) rbt \<Rightarrow> ('a, 'b) rbt" where
   "app RBT_Impl.Empty t = t"
 | "app t RBT_Impl.Empty = t"
-| "app (MR t1 a t2) (MR t3 c t4) = (case app t2 t3 of
-    MR u2 b u3 \<Rightarrow> (MR (MR t1 a u2) b (MR u3 c t4))
-  | t23 \<Rightarrow> MR t1 a (MR t23 c t4))"
-| "app (MB t1 a t2) (MB t3 c t4) = (case app t2 t3 of
-    MR u2 b u3 \<Rightarrow> MR (MB t1 a u2) b (MB u3 c t4)
-  | t23 \<Rightarrow> baldL t1 a (MB t23 c t4))"
-| "app t1 (MR t2 a t3) = MR (app t1 t2) a t3"
-| "app (MR t1 a t2) t3 = MR t1 a (app t2 t3)"
+| "app (MR t1 a b t2) (MR t3 a'' b'' t4) = (case app t2 t3 of
+    MR u2 a' b' u3 \<Rightarrow> (MR (MR t1 a b u2) a' b' (MR u3 a'' b'' t4))
+  | t23 \<Rightarrow> MR t1 a b (MR t23 a'' b'' t4))"
+| "app (MB t1 a b t2) (MB t3 a'' b'' t4) = (case app t2 t3 of
+    MR u2 a' b' u3 \<Rightarrow> MR (MB t1 a b u2) a' b' (MB u3 a'' b'' t4)
+  | t23 \<Rightarrow> baldL t1 a b (MB t23 a'' b'' t4))"
+| "app t1 (MR t2 a b t3) = MR (app t1 t2) a b t3"
+| "app (MR t1 a b t2) t3 = MR t1 a b (app t2 t3)"
 
-fun rbt_joinL :: "'a urbt \<Rightarrow> 'a \<Rightarrow> 'a urbt \<Rightarrow> 'a urbt" where
-  "rbt_joinL l x r = (if bheight l \<ge> bheight r then MR l x r
-    else case r of MB l' x' r' \<Rightarrow> baliL (rbt_joinL l x l') x' r'
-    | MR l' x' r' \<Rightarrow> MR (rbt_joinL l x l') x' r')"
+fun rbt_joinL :: "('a, 'b) rbt \<Rightarrow> 'a \<Rightarrow> 'b \<Rightarrow> ('a, 'b) rbt \<Rightarrow> ('a, 'b) rbt" where
+  "rbt_joinL l a b r = (if bheight l \<ge> bheight r then MR l a b r
+    else case r of MB l' a' b' r' \<Rightarrow> baliL (rbt_joinL l a b l') a' b' r'
+    | MR l' a' b' r' \<Rightarrow> MR (rbt_joinL l a b l') a' b' r')"
 
-fun rbt_joinR :: "'a urbt \<Rightarrow> 'a \<Rightarrow> 'a urbt \<Rightarrow> 'a urbt" where
-  "rbt_joinR l x r = (if bheight l \<le> bheight r then MR l x r
-    else case l of MB l' x' r' \<Rightarrow> baliR l' x' (rbt_joinR r' x r)
-    | MR l' x' r' \<Rightarrow> MR l' x' (rbt_joinR r' x r))"
+fun rbt_joinR :: "('a, 'b) rbt \<Rightarrow> 'a \<Rightarrow> 'b \<Rightarrow> ('a, 'b) rbt \<Rightarrow> ('a, 'b) rbt" where
+  "rbt_joinR l a b r = (if bheight l \<le> bheight r then MR l a b r
+    else case l of MB l' a' b' r' \<Rightarrow> baliR l' a' b' (rbt_joinR r' a b r)
+    | MR l' a' b' r' \<Rightarrow> MR l' a' b' (rbt_joinR r' a b r))"
 
-definition rbt_join :: "'a urbt \<Rightarrow> 'a \<Rightarrow> 'a urbt \<Rightarrow> 'a urbt" where
-  "rbt_join l x r = (if bheight l > bheight r
-    then paint RBT_Impl.B (rbt_joinR l x r)
+definition rbt_join :: "('a, 'b) rbt \<Rightarrow> 'a \<Rightarrow> 'b \<Rightarrow> ('a, 'b) rbt \<Rightarrow> ('a, 'b) rbt" where
+  "rbt_join l a b r = (if bheight l > bheight r
+    then paint RBT_Impl.B (rbt_joinR l a b r)
     else if bheight l < bheight r
-    then paint RBT_Impl.B (rbt_joinL l x r)
-    else MB l x r)"
+    then paint RBT_Impl.B (rbt_joinL l a b r)
+    else MB l a b r)"
 
 declare rbt_joinL.simps[simp del]
 declare rbt_joinR.simps[simp del]
@@ -80,36 +80,36 @@ declare rbt_joinR.simps[simp del]
 lemma [simp]: "size (paint c t) = size t"
   by (cases t) auto
 
-lemma size_baliL[simp]: "size (baliL t1 x t2) = Suc (size t1 + size t2)"
-  by (induction t1 x t2 rule: baliL.induct) auto
+lemma size_baliL[simp]: "size (baliL t1 a b t2) = Suc (size t1 + size t2)"
+  by (induction t1 a b t2 rule: baliL.induct) auto
 
-lemma size_baliR[simp]: "size (baliR t1 x t2) = Suc (size t1 + size t2)"
-  by (induction t1 x t2 rule: baliR.induct) auto
+lemma size_baliR[simp]: "size (baliR t1 a b t2) = Suc (size t1 + size t2)"
+  by (induction t1 a b t2 rule: baliR.induct) auto
 
-lemma size_baldL[simp]: "size (baldL t1 x t2) = Suc (size t1 + size t2)"
-  by (induction t1 x t2 rule: baldL.induct) auto
+lemma size_baldL[simp]: "size (baldL t1 a b t2) = Suc (size t1 + size t2)"
+  by (induction t1 a b t2 rule: baldL.induct) auto
 
-lemma size_baldR[simp]: "size (baldR t1 x t2) = Suc (size t1 + size t2)"
-  by (induction t1 x t2 rule: baldR.induct) auto
+lemma size_baldR[simp]: "size (baldR t1 a b t2) = Suc (size t1 + size t2)"
+  by (induction t1 a b t2 rule: baldR.induct) auto
 
 lemma size_app[simp]: "size (app t1 t2) = size t1 + size t2"
   by (induction t1 t2 rule: app.induct)
      (auto split: RBT_Impl.rbt.splits RBT_Impl.color.splits unit.splits)
 
-lemma size_rbt_joinL[simp]: "size (rbt_joinL t1 x t2) = Suc (size t1 + size t2)"
-  by (induction t1 x t2 rule: rbt_joinL.induct)
+lemma size_rbt_joinL[simp]: "size (rbt_joinL t1 a b t2) = Suc (size t1 + size t2)"
+  by (induction t1 a b t2 rule: rbt_joinL.induct)
      (auto simp: rbt_joinL.simps split: RBT_Impl.rbt.splits RBT_Impl.color.splits unit.splits)
 
-lemma size_rbt_joinR[simp]: "size (rbt_joinR t1 x t2) = Suc (size t1 + size t2)"
-  by (induction t1 x t2 rule: rbt_joinR.induct)
+lemma size_rbt_joinR[simp]: "size (rbt_joinR t1 a b t2) = Suc (size t1 + size t2)"
+  by (induction t1 a b t2 rule: rbt_joinR.induct)
      (auto simp: rbt_joinR.simps split: RBT_Impl.rbt.splits RBT_Impl.color.splits unit.splits)
 
-lemma size_rbt_join[simp]: "size (rbt_join t1 x t2) = Suc (size t1 + size t2)"
+lemma size_rbt_join[simp]: "size (rbt_join t1 a b t2) = Suc (size t1 + size t2)"
   by (auto simp: rbt_join_def)
 
 definition "rbt t \<longleftrightarrow> inv1 t \<and> inv2 t"
 
-lemma rbt_Node: "\<lbrakk> rbt (RBT_Impl.Branch c l a () r) \<rbrakk> \<Longrightarrow> rbt l \<and> rbt r"
+lemma rbt_Node: "\<lbrakk> rbt (RBT_Impl.Branch c l a b r) \<rbrakk> \<Longrightarrow> rbt l \<and> rbt r"
   by (auto simp: rbt_def)
 
 lemma color_of_paint_B: "color_of (paint RBT_Impl.B t) = RBT_Impl.B"
@@ -125,36 +125,36 @@ lemma inv2_paint: "inv2 t \<Longrightarrow> inv2 (paint c t)"
   by (cases t) auto
 
 lemma inv1_baliL:
-  "\<lbrakk>inv1l l; inv1 r\<rbrakk> \<Longrightarrow> inv1 (baliL l a r)"
-  by (induct l a r rule: baliL.induct) auto
+  "\<lbrakk>inv1l l; inv1 r\<rbrakk> \<Longrightarrow> inv1 (baliL l a b r)"
+  by (induct l a b r rule: baliL.induct) auto
 
 lemma inv1_baliR:
-  "\<lbrakk>inv1 l; inv1l r\<rbrakk> \<Longrightarrow> inv1 (baliR l a r)"
-  by (induct l a r rule: baliR.induct) auto
+  "\<lbrakk>inv1 l; inv1l r\<rbrakk> \<Longrightarrow> inv1 (baliR l a b r)"
+  by (induct l a b r rule: baliR.induct) auto
 
 lemma bheight_baliL:
-  "bheight l = bheight r \<Longrightarrow> bheight (baliL l a r) = Suc (bheight l)"
-  by (induct l a r rule: baliL.induct) auto
+  "bheight l = bheight r \<Longrightarrow> bheight (baliL l a b r) = Suc (bheight l)"
+  by (induct l a b r rule: baliL.induct) auto
 
 lemma bheight_baliR:
-  "bheight l = bheight r \<Longrightarrow> bheight (baliR l a r) = Suc (bheight l)"
-  by (induct l a r rule: baliR.induct) auto
+  "bheight l = bheight r \<Longrightarrow> bheight (baliR l a b r) = Suc (bheight l)"
+  by (induct l a b r rule: baliR.induct) auto
 
 lemma inv2_baliL:
-  "\<lbrakk> inv2 l; inv2 r; bheight l = bheight r \<rbrakk> \<Longrightarrow> inv2 (baliL l a r)"
-  by (induct l a r rule: baliL.induct) auto
+  "\<lbrakk> inv2 l; inv2 r; bheight l = bheight r \<rbrakk> \<Longrightarrow> inv2 (baliL l a b r)"
+  by (induct l a b r rule: baliL.induct) auto
 
 lemma inv2_baliR:
-  "\<lbrakk> inv2 l; inv2 r; bheight l = bheight r \<rbrakk> \<Longrightarrow> inv2 (baliR l a r)"
-  by (induct l a r rule: baliR.induct) auto
+  "\<lbrakk> inv2 l; inv2 r; bheight l = bheight r \<rbrakk> \<Longrightarrow> inv2 (baliR l a b r)"
+  by (induct l a b r rule: baliR.induct) auto
 
 lemma inv_baliR: "\<lbrakk> inv2 l; inv2 r; inv1 l; inv1l r; bheight l = bheight r \<rbrakk>
- \<Longrightarrow> inv1 (baliR l a r) \<and> inv2 (baliR l a r) \<and> bheight (baliR l a r) = Suc (bheight l)"
-  by (induct l a r rule: baliR.induct) auto
+ \<Longrightarrow> inv1 (baliR l a b r) \<and> inv2 (baliR l a b r) \<and> bheight (baliR l a b r) = Suc (bheight l)"
+  by (induct l a b r rule: baliR.induct) auto
 
 lemma inv_baliL: "\<lbrakk> inv2 l; inv2 r; inv1l l; inv1 r; bheight l = bheight r \<rbrakk>
- \<Longrightarrow> inv1 (baliL l a r) \<and> inv2 (baliL l a r) \<and> bheight (baliL l a r) = Suc (bheight l)"
-  by (induct l a r rule: baliL.induct) auto
+ \<Longrightarrow> inv1 (baliL l a b r) \<and> inv2 (baliL l a b r) \<and> bheight (baliL l a b r) = Suc (bheight l)"
+  by (induct l a b r rule: baliL.induct) auto
 
 lemma bheight_paint_R:
   "color_of t = RBT_Impl.B \<Longrightarrow> bheight (paint RBT_Impl.R t) = bheight t - 1"
@@ -162,17 +162,17 @@ lemma bheight_paint_R:
 
 lemma inv2_baldL_inv1:
   "\<lbrakk> inv2 l;  inv2 r;  bheight l + 1 = bheight r;  inv1 r \<rbrakk>
-   \<Longrightarrow> inv2 (baldL l a r) \<and> bheight (baldL l a r) = bheight r"
-  by (induct l a r rule: baldL.induct)
+   \<Longrightarrow> inv2 (baldL l a b r) \<and> bheight (baldL l a b r) = bheight r"
+  by (induct l a b r rule: baldL.induct)
      (auto simp: inv2_baliR inv2_paint bheight_baliR bheight_paint_R)
 
 lemma inv2_baldL_B:
   "\<lbrakk> inv2 l;  inv2 r;  bheight l + 1 = bheight r; color_of r = RBT_Impl.B \<rbrakk>
-   \<Longrightarrow> inv2 (baldL l a r) \<and> bheight (baldL l a r) = bheight r"
-  by (induct l a r rule: baldL.induct) (auto simp add: inv2_baliR bheight_baliR)
+   \<Longrightarrow> inv2 (baldL l a b r) \<and> bheight (baldL l a b r) = bheight r"
+  by (induct l a b r rule: baldL.induct) (auto simp add: inv2_baliR bheight_baliR)
 
-lemma inv1_baldL: "\<lbrakk>inv1l l; inv1 r; color_of r = RBT_Impl.B\<rbrakk> \<Longrightarrow> inv1 (baldL l a r)"
-  by (induct l a r rule: baldL.induct) (simp_all add: inv1_baliR)
+lemma inv1_baldL: "\<lbrakk>inv1l l; inv1 r; color_of r = RBT_Impl.B\<rbrakk> \<Longrightarrow> inv1 (baldL l a b r)"
+  by (induct l a b r rule: baldL.induct) (simp_all add: inv1_baliR)
 
 lemma inv1lI: "inv1 t \<Longrightarrow> inv1l t"
   by (cases t) auto
@@ -183,20 +183,20 @@ lemma neq_Black[simp]: "(c \<noteq> RBT_Impl.B) = (c = RBT_Impl.R)"
 lemma [simp]: "inv1 t \<Longrightarrow> inv1l (paint c t)"
   by (cases t) auto
 
-lemma inv1l_baldL: "\<lbrakk> inv1l l; inv1 r \<rbrakk> \<Longrightarrow> inv1l (baldL l a r)"
-  by (induct l a r rule: baldL.induct) (auto simp: inv1_baliR paint2)
+lemma inv1l_baldL: "\<lbrakk> inv1l l; inv1 r \<rbrakk> \<Longrightarrow> inv1l (baldL l a b r)"
+  by (induct l a b r rule: baldL.induct) (auto simp: inv1_baliR paint2)
 
 lemma inv2_baldR_inv1:
   "\<lbrakk> inv2 l;  inv2 r;  bheight l = bheight r + 1;  inv1 l \<rbrakk>
-  \<Longrightarrow> inv2 (baldR l a r) \<and> bheight (baldR l a r) = bheight l"
-  by (induct l a r rule: baldR.induct)
+  \<Longrightarrow> inv2 (baldR l a b r) \<and> bheight (baldR l a b r) = bheight l"
+  by (induct l a b r rule: baldR.induct)
      (auto simp: inv2_baliL bheight_baliL inv2_paint bheight_paint_R)
 
-lemma inv1_baldR: "\<lbrakk>inv1 l; inv1l r; color_of l = RBT_Impl.B\<rbrakk> \<Longrightarrow> inv1 (baldR l a r)"
-  by (induct l a r rule: baldR.induct) (simp_all add: inv1_baliL)
+lemma inv1_baldR: "\<lbrakk>inv1 l; inv1l r; color_of l = RBT_Impl.B\<rbrakk> \<Longrightarrow> inv1 (baldR l a b r)"
+  by (induct l a b r rule: baldR.induct) (simp_all add: inv1_baliL)
 
-lemma inv1l_baldR: "\<lbrakk> inv1 l; inv1l r \<rbrakk> \<Longrightarrow>inv1l (baldR l a r)"
-  by (induct l a r rule: baldR.induct) (auto simp: inv1_baliL paint2)
+lemma inv1l_baldR: "\<lbrakk> inv1 l; inv1l r \<rbrakk> \<Longrightarrow>inv1l (baldR l a b r)"
+  by (induct l a b r rule: baldR.induct) (auto simp: inv1_baliL paint2)
 
 lemma inv2_app:
   "\<lbrakk> inv2 l; inv2 r; bheight l = bheight r \<rbrakk>
@@ -212,16 +212,16 @@ lemma inv1_app:
 
 lemma inv_baldL:
   "\<lbrakk> inv2 l;  inv2 r;  bheight l + 1 = bheight r; inv1l l; inv1 r \<rbrakk>
-   \<Longrightarrow> inv2 (baldL l a r) \<and> bheight (baldL l a r) = bheight r
-  \<and> inv1l (baldL l a r) \<and> (color_of r = RBT_Impl.B \<longrightarrow> inv1 (baldL l a r))"
-  by (induct l a r rule: baldL.induct)
+   \<Longrightarrow> inv2 (baldL l a b r) \<and> bheight (baldL l a b r) = bheight r
+  \<and> inv1l (baldL l a b r) \<and> (color_of r = RBT_Impl.B \<longrightarrow> inv1 (baldL l a b r))"
+  by (induct l a b r rule: baldL.induct)
      (auto simp: inv_baliR inv2_paint bheight_baliR bheight_paint_R paint2)
 
 lemma inv_baldR:
   "\<lbrakk> inv2 l;  inv2 r;  bheight l = bheight r + 1; inv1 l; inv1l r \<rbrakk>
-   \<Longrightarrow> inv2 (baldR l a r) \<and> bheight (baldR l a r) = bheight l
-  \<and> inv1l (baldR l a r) \<and> (color_of l = RBT_Impl.B \<longrightarrow> inv1 (baldR l a r))"
-  by (induct l a r rule: baldR.induct)
+   \<Longrightarrow> inv2 (baldR l a b r) \<and> bheight (baldR l a b r) = bheight l
+  \<and> inv1l (baldR l a b r) \<and> (color_of l = RBT_Impl.B \<longrightarrow> inv1 (baldR l a b r))"
+  by (induct l a b r rule: baldR.induct)
      (auto simp: inv_baliL inv2_paint bheight_baliL bheight_paint_R paint2)
 
 lemma inv_app:
@@ -237,53 +237,53 @@ lemma neq_LeafD: "t \<noteq> RBT_Impl.Empty \<Longrightarrow> \<exists>l x c r. 
 
 lemma inv1l_rbt_joinL:
  "\<lbrakk> inv1 l; inv1 r; bheight l \<le> bheight r \<rbrakk> \<Longrightarrow>
-  inv1l (rbt_joinL l x r)
-  \<and> (bheight l \<noteq> bheight r \<and> color_of r = RBT_Impl.B \<longrightarrow> inv1(rbt_joinL l x r))"
-proof (induct l x r rule: rbt_joinL.induct)
-  case (1 l x r) thus ?case
-    by (auto simp: inv1_baliL rbt_joinL.simps[of l x r]
+  inv1l (rbt_joinL l a b r)
+  \<and> (bheight l \<noteq> bheight r \<and> color_of r = RBT_Impl.B \<longrightarrow> inv1(rbt_joinL l a b r))"
+proof (induct l a b r rule: rbt_joinL.induct)
+  case (1 l a b r) thus ?case
+    by (auto simp: inv1_baliL rbt_joinL.simps[of l a b r]
         split!: RBT_Impl.rbt.splits RBT_Impl.color.splits unit.splits)
 qed
 
 lemma inv1l_rbt_joinR:
   "\<lbrakk> inv1 l; inv2 l; inv1 r; inv2 r; bheight l \<ge> bheight r \<rbrakk> \<Longrightarrow>
-  inv1l (rbt_joinR l x r)
-  \<and> (bheight l \<noteq> bheight r \<and> color_of l = RBT_Impl.B \<longrightarrow> inv1(rbt_joinR l x r))"
-proof (induct l x r rule: rbt_joinR.induct)
-  case (1 l x r) thus ?case
-    by (fastforce simp: inv1_baliR rbt_joinR.simps[of l x r]
+  inv1l (rbt_joinR l a b r)
+  \<and> (bheight l \<noteq> bheight r \<and> color_of l = RBT_Impl.B \<longrightarrow> inv1(rbt_joinR l a b r))"
+proof (induct l a b r rule: rbt_joinR.induct)
+  case (1 l a b r) thus ?case
+    by (fastforce simp: inv1_baliR rbt_joinR.simps[of l a b r]
         split!: RBT_Impl.rbt.splits RBT_Impl.color.splits unit.splits)
 qed
 
 lemma bheight_rbt_joinL:
-  "\<lbrakk> inv2 l; inv2 r; bheight l \<le> bheight r \<rbrakk> \<Longrightarrow> bheight (rbt_joinL l x r) = bheight r"
-proof (induct l x r rule: rbt_joinL.induct)
-  case (1 l x r) thus ?case
-    by (auto simp: bheight_baliL rbt_joinL.simps[of l x r]
+  "\<lbrakk> inv2 l; inv2 r; bheight l \<le> bheight r \<rbrakk> \<Longrightarrow> bheight (rbt_joinL l a b r) = bheight r"
+proof (induct l a b r rule: rbt_joinL.induct)
+  case (1 l a b r) thus ?case
+    by (auto simp: bheight_baliL rbt_joinL.simps[of l a b r]
         split!: RBT_Impl.rbt.splits RBT_Impl.color.splits unit.splits)
 qed
 
 lemma inv2_rbt_joinL:
-  "\<lbrakk> inv2 l;  inv2 r;  bheight l \<le> bheight r \<rbrakk> \<Longrightarrow> inv2 (rbt_joinL l x r)"
-proof (induct l x r rule: rbt_joinL.induct)
-  case (1 l x r) thus ?case
-    by (auto simp: inv2_baliL bheight_rbt_joinL rbt_joinL.simps[of l x r]
+  "\<lbrakk> inv2 l;  inv2 r;  bheight l \<le> bheight r \<rbrakk> \<Longrightarrow> inv2 (rbt_joinL l a b r)"
+proof (induct l a b r rule: rbt_joinL.induct)
+  case (1 l a b r) thus ?case
+    by (auto simp: inv2_baliL bheight_rbt_joinL rbt_joinL.simps[of l a b r]
         split!: RBT_Impl.rbt.splits RBT_Impl.color.splits unit.splits)
 qed
 
 lemma bheight_rbt_joinR:
-  "\<lbrakk> inv2 l;  inv2 r;  bheight l \<ge> bheight r \<rbrakk> \<Longrightarrow> bheight (rbt_joinR l x r) = bheight l"
-proof (induct l x r rule: rbt_joinR.induct)
-  case (1 l x r) thus ?case
-    by (fastforce simp: bheight_baliR rbt_joinR.simps[of l x r]
+  "\<lbrakk> inv2 l;  inv2 r;  bheight l \<ge> bheight r \<rbrakk> \<Longrightarrow> bheight (rbt_joinR l a b r) = bheight l"
+proof (induct l a b r rule: rbt_joinR.induct)
+  case (1 l a b r) thus ?case
+    by (fastforce simp: bheight_baliR rbt_joinR.simps[of l a b r]
         split!: RBT_Impl.rbt.splits RBT_Impl.color.splits unit.splits)
 qed
 
 lemma inv2_rbt_joinR:
-  "\<lbrakk> inv2 l; inv2 r; bheight l \<ge> bheight r \<rbrakk> \<Longrightarrow> inv2 (rbt_joinR l x r)"
-proof (induct l x r rule: rbt_joinR.induct)
-  case (1 l x r) thus ?case
-    by (fastforce simp: inv2_baliR bheight_rbt_joinR rbt_joinR.simps[of l x r]
+  "\<lbrakk> inv2 l; inv2 r; bheight l \<ge> bheight r \<rbrakk> \<Longrightarrow> inv2 (rbt_joinR l a b r)"
+proof (induct l a b r rule: rbt_joinR.induct)
+  case (1 l a b r) thus ?case
+    by (fastforce simp: inv2_baliR bheight_rbt_joinR rbt_joinR.simps[of l a b r]
         split!: RBT_Impl.rbt.splits RBT_Impl.color.splits unit.splits)
 qed
 
@@ -294,21 +294,21 @@ lemma keys_paint: "RBT_Impl.keys (paint c t) = RBT_Impl.keys t"
   by (cases t) auto
 
 lemma keys_baliL:
-  "RBT_Impl.keys (baliL l a r) = RBT_Impl.keys l @ a # RBT_Impl.keys r"
-  by (cases "(l,a,r)" rule: baliL.cases) auto
+  "RBT_Impl.keys (baliL l a b r) = RBT_Impl.keys l @ a # RBT_Impl.keys r"
+  by (cases "(l,a,b,r)" rule: baliL.cases) auto
 
 lemma keys_baliR:
-  "RBT_Impl.keys (baliR l a r) = RBT_Impl.keys l @ a # RBT_Impl.keys r"
-  by (cases "(l,a,r)" rule: baliR.cases) auto
+  "RBT_Impl.keys (baliR l a b r) = RBT_Impl.keys l @ a # RBT_Impl.keys r"
+  by (cases "(l,a,b,r)" rule: baliR.cases) auto
 
 lemma keys_baldL:
-  "RBT_Impl.keys (baldL l a r) = RBT_Impl.keys l @ a # RBT_Impl.keys r"
-  by (cases "(l,a,r)" rule: baldL.cases)
+  "RBT_Impl.keys (baldL l a b r) = RBT_Impl.keys l @ a # RBT_Impl.keys r"
+  by (cases "(l,a,b,r)" rule: baldL.cases)
      (auto simp: keys_baliL keys_baliR keys_paint)
 
 lemma keys_baldR:
-  "RBT_Impl.keys (baldR l a r) = RBT_Impl.keys l @ a # RBT_Impl.keys r"
-  by (cases "(l,a,r)" rule: baldR.cases)
+  "RBT_Impl.keys (baldR l a b r) = RBT_Impl.keys l @ a # RBT_Impl.keys r"
+  by (cases "(l,a,b,r)" rule: baldR.cases)
      (auto simp: keys_baliL keys_baliR keys_paint)
 
 lemma keys_app:
@@ -318,70 +318,70 @@ lemma keys_app:
       split: RBT_Impl.rbt.splits RBT_Impl.color.splits unit.splits)
 
 lemma keys_rbt_joinL: "bheight l \<le> bheight r \<Longrightarrow>
-  RBT_Impl.keys (rbt_joinL l x r) = RBT_Impl.keys l @ x # RBT_Impl.keys r"
-proof (induction l x r rule: rbt_joinL.induct)
-  case (1 l x r)
+  RBT_Impl.keys (rbt_joinL l a b r) = RBT_Impl.keys l @ a # RBT_Impl.keys r"
+proof (induction l a b r rule: rbt_joinL.induct)
+  case (1 l a b r)
   thus ?case
-    by (auto simp: keys_baliL rbt_joinL.simps[of l x r]
+    by (auto simp: keys_baliL rbt_joinL.simps[of l a b r]
         split!: RBT_Impl.rbt.splits RBT_Impl.color.splits unit.splits)
 qed
 
 lemma keys_rbt_joinR:
-  "RBT_Impl.keys (rbt_joinR l x r) = RBT_Impl.keys l @ x # RBT_Impl.keys r"
-proof (induction l x r rule: rbt_joinR.induct)
-  case (1 l x r)
+  "RBT_Impl.keys (rbt_joinR l a b r) = RBT_Impl.keys l @ a # RBT_Impl.keys r"
+proof (induction l a b r rule: rbt_joinR.induct)
+  case (1 l a b r)
   thus ?case
-    by (force simp: keys_baliR rbt_joinR.simps[of l x r]
+    by (force simp: keys_baliR rbt_joinR.simps[of l a b r]
         split!: RBT_Impl.rbt.splits RBT_Impl.color.splits unit.splits)
 qed
 
 lemma set_baliL:
-  "set (RBT_Impl.keys (baliL l a r)) = set (RBT_Impl.keys l) \<union> {a} \<union> set (RBT_Impl.keys r)"
-  by (cases "(l,a,r)" rule: baliL.cases) auto
+  "set (RBT_Impl.keys (baliL l a b r)) = set (RBT_Impl.keys l) \<union> {a} \<union> set (RBT_Impl.keys r)"
+  by (cases "(l,a,b,r)" rule: baliL.cases) auto
 
 lemma set_rbt_joinL:
   "bheight l \<le> bheight r \<Longrightarrow>
-  set (RBT_Impl.keys (rbt_joinL l x r)) = set (RBT_Impl.keys l) \<union> {x} \<union> set (RBT_Impl.keys r)"
-proof (induction l x r rule: rbt_joinL.induct)
-  case (1 l x r)
+  set (RBT_Impl.keys (rbt_joinL l a b r)) = set (RBT_Impl.keys l) \<union> {a} \<union> set (RBT_Impl.keys r)"
+proof (induction l a b r rule: rbt_joinL.induct)
+  case (1 l a b r)
   thus ?case
-    by (auto simp: set_baliL rbt_joinL.simps[of l x r]
+    by (auto simp: set_baliL rbt_joinL.simps[of l a b r]
         split!: RBT_Impl.rbt.splits RBT_Impl.color.splits unit.splits)
 qed
 
 lemma set_baliR:
-  "set (RBT_Impl.keys (baliR l a r)) = set (RBT_Impl.keys l) \<union> {a} \<union> set (RBT_Impl.keys r)"
-  by (cases "(l,a,r)" rule: baliR.cases) auto
+  "set (RBT_Impl.keys (baliR l a b r)) = set (RBT_Impl.keys l) \<union> {a} \<union> set (RBT_Impl.keys r)"
+  by (cases "(l,a,b,r)" rule: baliR.cases) auto
 
 lemma set_rbt_joinR:
-  "set (RBT_Impl.keys (rbt_joinR l x r)) = set (RBT_Impl.keys l) \<union> {x} \<union> set (RBT_Impl.keys r)"
-proof (induction l x r rule: rbt_joinR.induct)
-  case (1 l x r)
+  "set (RBT_Impl.keys (rbt_joinR l a b r)) = set (RBT_Impl.keys l) \<union> {a} \<union> set (RBT_Impl.keys r)"
+proof (induction l a b r rule: rbt_joinR.induct)
+  case (1 l a b r)
   thus ?case
-    by (force simp: set_baliR rbt_joinR.simps[of l x r]
+    by (force simp: set_baliR rbt_joinR.simps[of l a b r]
         split!: RBT_Impl.rbt.splits RBT_Impl.color.splits unit.splits)
 qed
 
 lemma set_paint: "set (RBT_Impl.keys (paint c t)) = set (RBT_Impl.keys t)"
   by (cases t) auto
 
-lemma set_rbt_join: "set (RBT_Impl.keys (rbt_join l x r)) =
-  set (RBT_Impl.keys l) \<union> {x} \<union> set (RBT_Impl.keys r)"
+lemma set_rbt_join: "set (RBT_Impl.keys (rbt_join l a b r)) =
+  set (RBT_Impl.keys l) \<union> {a} \<union> set (RBT_Impl.keys r)"
   by (simp add: set_rbt_joinL set_rbt_joinR set_paint rbt_join_def)
 
 lemma inv_rbt_join: "\<lbrakk> inv1 l; inv2 l; inv1 r; inv2 r \<rbrakk> \<Longrightarrow>
-  inv1 (rbt_join l x r) \<and> inv2 (rbt_join l x r)"
+  inv1 (rbt_join l a b r) \<and> inv2 (rbt_join l a b r)"
   by (auto simp: rbt_join_def inv1l_rbt_joinL inv1l_rbt_joinR inv2_rbt_joinL inv2_rbt_joinR
       inv2_paint inv1_paint_B)
 
-lemma color_of_rbt_join: "color_of (rbt_join l x r) = color.B"
+lemma color_of_rbt_join: "color_of (rbt_join l a b r) = color.B"
   by (auto simp: rbt_join_def color_of_paint_B)
 
-lemma rbt_join: "rbt l \<Longrightarrow> rbt r \<Longrightarrow> rbt (rbt_join l x r)"
+lemma rbt_join: "rbt l \<Longrightarrow> rbt r \<Longrightarrow> rbt (rbt_join l a b r)"
   using inv_rbt_join
   by (fastforce simp: rbt_def color_of_rbt_join)
 
-fun rbt_recolor :: "('a, unit) rbt \<Rightarrow> ('a, unit) rbt" where
+fun rbt_recolor :: "('a, 'b) rbt \<Rightarrow> ('a, 'b) rbt" where
   "rbt_recolor (Branch RBT_Impl.R t1 k v t2) =
     (if color_of t1 = RBT_Impl.B \<and> color_of t2 = RBT_Impl.B then Branch RBT_Impl.B t1 k v t2
     else Branch RBT_Impl.R t1 k v t2)"
@@ -390,22 +390,22 @@ fun rbt_recolor :: "('a, unit) rbt \<Rightarrow> ('a, unit) rbt" where
 lemma rbt_recolor: "rbt t \<Longrightarrow> rbt (rbt_recolor t)"
   by (induction t rule: rbt_recolor.induct) (auto simp: rbt_def)
 
-fun split_min :: "'a urbt \<Rightarrow> 'a \<times> 'a urbt" where
+fun split_min :: "('a, 'b) rbt \<Rightarrow> 'a \<times> 'b \<times> ('a, 'b) rbt" where
   "split_min RBT_Impl.Empty = undefined"
-| "split_min (RBT_Impl.Branch _ l a _ r) =
-    (if is_empty l then (a,r) else let (m, l') = split_min l in (m, rbt_join l' a r))"
+| "split_min (RBT_Impl.Branch _ l a b r) =
+    (if is_empty l then (a,b,r) else let (a',b',l') = split_min l in (a',b',rbt_join l' a b r))"
 
 lemma split_min_set:
-  "\<lbrakk> split_min t = (m,t');  t \<noteq> RBT_Impl.Empty \<rbrakk> \<Longrightarrow>
-  m \<in> set (RBT_Impl.keys t) \<and> set (RBT_Impl.keys t) = {m} \<union> set (RBT_Impl.keys t')"
+  "\<lbrakk> split_min t = (a,b,t');  t \<noteq> RBT_Impl.Empty \<rbrakk> \<Longrightarrow>
+  a \<in> set (RBT_Impl.keys t) \<and> set (RBT_Impl.keys t) = {a} \<union> set (RBT_Impl.keys t')"
   by (induction t arbitrary: t') (auto simp: set_rbt_join split: prod.splits if_splits)
 
 lemma split_min_inv:
-  "\<lbrakk> split_min t = (m,t');  rbt t;  t \<noteq> RBT_Impl.Empty \<rbrakk> \<Longrightarrow> rbt t'"
+  "\<lbrakk> split_min t = (a,b,t');  rbt t;  t \<noteq> RBT_Impl.Empty \<rbrakk> \<Longrightarrow> rbt t'"
   by (induction t arbitrary: t') (auto simp: rbt_join split: if_splits prod.splits dest: rbt_Node)
 
-definition rbt_join2 :: "'a urbt \<Rightarrow> 'a urbt \<Rightarrow> 'a urbt" where
-  "rbt_join2 l r = (if is_empty r then l else let (m, r') = split_min r in rbt_join l m r')"
+definition rbt_join2 :: "('a, 'b) rbt \<Rightarrow> ('a, 'b) rbt \<Rightarrow> ('a, 'b) rbt" where
+  "rbt_join2 l r = (if is_empty r then l else let (a,b,r') = split_min r in rbt_join l a b r')"
 
 lemma set_rbt_join2[simp]:
   "set (RBT_Impl.keys (rbt_join2 l r)) = set (RBT_Impl.keys l) \<union> set (RBT_Impl.keys r)"
@@ -416,30 +416,32 @@ lemma inv_rbt_join2: "\<lbrakk> rbt l; rbt r \<rbrakk> \<Longrightarrow> rbt (rb
 
 context ord begin
 
-fun split :: "'a urbt \<Rightarrow> 'a \<Rightarrow> 'a urbt \<times> bool \<times> 'a urbt" where
-  "split RBT_Impl.Empty k = (RBT_Impl.Empty, False, RBT_Impl.Empty)"
-| "split (RBT_Impl.Branch _ l a () r) x =
-  (if x < a then (case split l x of (l1, b, l2) \<Rightarrow> (l1, b, rbt_join l2 a r))
-  else if a < x then (case split r x of (r1, b, r2) \<Rightarrow> (rbt_join l a r1, b, r2))
-  else (l, True, r))"
+fun split :: "('a, 'b) rbt \<Rightarrow> 'a \<Rightarrow> ('a, 'b) rbt \<times> 'b option \<times> ('a, 'b) rbt" where
+  "split RBT_Impl.Empty k = (RBT_Impl.Empty, None, RBT_Impl.Empty)"
+| "split (RBT_Impl.Branch _ l a b r) x =
+  (if x < a then (case split l x of (l1, \<beta>, l2) \<Rightarrow> (l1, \<beta>, rbt_join l2 a b r))
+  else if a < x then (case split r x of (r1, \<beta>, r2) \<Rightarrow> (rbt_join l a b r1, \<beta>, r2))
+  else (l, Some b, r))"
 
-lemma split_rbt: "split t x = (l,xin,r) \<Longrightarrow> rbt t \<Longrightarrow> rbt l \<and> rbt r"
-  by (induction t arbitrary: l xin r)
+lemma split_rbt: "split t x = (l,\<beta>,r) \<Longrightarrow> rbt t \<Longrightarrow> rbt l \<and> rbt r"
+  by (induction t arbitrary: l r)
      (auto simp: set_rbt_join rbt_join rbt_greater_prop rbt_less_prop
       split: if_splits prod.splits dest!: rbt_Node)
 
-lemma split_size: "split t2 a = (l2, b, r2) \<Longrightarrow> size l2 + size r2 \<le> size t2"
-  by (induction t2 a arbitrary: l2 b r2 rule: split.induct) (auto split: if_splits prod.splits)
+lemma split_size: "split t2 a = (l2,\<beta>,r2) \<Longrightarrow> size l2 + size r2 \<le> size t2"
+  by (induction t2 a arbitrary: l2 r2 rule: split.induct) (auto split: if_splits prod.splits)
 
-function union :: "'a urbt \<Rightarrow> 'a urbt \<Rightarrow> 'a urbt" where
-  "union t1 t2 = (let (t1, t2) = if flip_rbt t1 t2 then (t2, t1) else (t1, t2) in
-    if small_rbt t1 then RBT_Impl.fold rbt_insert t1 t2
+function union :: "('a \<Rightarrow> 'b \<Rightarrow> 'b \<Rightarrow> 'b) \<Rightarrow> ('a, 'b) rbt \<Rightarrow> ('a, 'b) rbt \<Rightarrow> ('a, 'b) rbt" where
+  "union f t1 t2 = (let (f, t1, t2) =
+    if flip_rbt t1 t2 then (\<lambda>k v v'. f k v' v, t2, t1) else (f, t1, t2) in
+    if small_rbt t1 then RBT_Impl.fold (rbt_insert_with_key f) t1 t2
     else (case t2 of RBT_Impl.Empty \<Rightarrow> t1
-      | RBT_Impl.Branch _ l2 a () r2 \<Rightarrow>
-        case split t1 a of (l1, _, r1) \<Rightarrow> rbt_join (union l1 l2) a (union r1 r2)))"
+      | RBT_Impl.Branch _ l2 a b r2 \<Rightarrow>
+        case split t1 a of (l1, \<beta>, r1) \<Rightarrow>
+          rbt_join (union f l1 l2) a (case \<beta> of None \<Rightarrow> b | Some b' \<Rightarrow> f a b b') (union f r1 r2)))"
   by pat_completeness auto
 termination
-  apply (relation "measure (\<lambda>(t1, t2). size t1 + size t2)")
+  apply (relation "measure (\<lambda>(f,t1, t2). size t1 + size t2)")
     apply (auto split: if_splits)
      apply (metis add_leD1 le_imp_less_Suc ord.split_size trans_le_add2)
     apply (metis add_leD1 le_imp_less_Suc ord.split_size trans_le_add1)
@@ -451,17 +453,17 @@ declare union.simps[simp del]
 
 lemma rbt_fold_rbt_insert:
   assumes "rbt t2"
-  shows "rbt (RBT_Impl.fold rbt_insert t1 t2)"
+  shows "rbt (RBT_Impl.fold (rbt_insert_with_key f) t1 t2)"
 proof -
   define xs where "xs = RBT_Impl.entries t1"
   from assms show ?thesis
     unfolding RBT_Impl.fold_def xs_def[symmetric]
     by (induct xs rule: rev_induct)
-       (auto simp: rbt_def rbt_insert_def rbt_insert_with_key_def ins_inv1_inv2)
+       (auto simp: rbt_def rbt_insert_with_key_def ins_inv1_inv2)
 qed
 
-lemma rbt_union: "rbt t1 \<Longrightarrow> rbt t2 \<Longrightarrow> rbt (union t1 t2)"
-proof (induction t1 t2 rule: union.induct)
+lemma rbt_union: "rbt t1 \<Longrightarrow> rbt t2 \<Longrightarrow> rbt (union f t1 t2)"
+proof (induction f t1 t2 rule: union.induct)
   case (1 t1 t2)
   thus ?case
     by (auto simp: union.simps[of t1 t2] rbt_join split_rbt rbt_fold_rbt_insert
@@ -469,17 +471,19 @@ proof (induction t1 t2 rule: union.induct)
         dest: rbt_Node)
 qed
 
-function inter :: "'a urbt \<Rightarrow> 'a urbt \<Rightarrow> 'a urbt" where
-  "inter t1 t2 = (let (t1, t2) = if flip_rbt t1 t2 then (t2, t1) else (t1, t2) in
+function inter :: "('a \<Rightarrow> 'b \<Rightarrow> 'b \<Rightarrow> 'b) \<Rightarrow> ('a, 'b) rbt \<Rightarrow> ('a, 'b) rbt \<Rightarrow> ('a, 'b) rbt" where
+  "inter f t1 t2 = (let (f, t1, t2) =
+    if flip_rbt t1 t2 then (\<lambda>k v v'. f k v' v, t2, t1) else (f, t1, t2) in
     if small_rbt t1 then
-      rbtreeify (filter (\<lambda>(k, _). rbt_lookup t2 k = Some ()) (RBT_Impl.entries t1))
+      rbtreeify (List.map_filter (\<lambda>(k, v). case rbt_lookup t2 k of None \<Rightarrow> None
+      | Some v' \<Rightarrow> Some (k, f k v v')) (RBT_Impl.entries t1))
     else case t2 of RBT_Impl.Empty \<Rightarrow> RBT_Impl.Empty
-    | RBT_Impl.Branch _ l2 a () r2 \<Rightarrow>
-      case split t1 a of (l1, ain, r1) \<Rightarrow> let l' = inter l1 l2; r' = inter r1 r2
-      in if ain then rbt_join l' a r' else rbt_join2 l' r')"
+    | RBT_Impl.Branch _ l2 a b r2 \<Rightarrow>
+      case split t1 a of (l1, \<beta>, r1) \<Rightarrow> let l' = inter f l1 l2; r' = inter f r1 r2 in
+      (case \<beta> of None \<Rightarrow> rbt_join2 l' r' | Some b' \<Rightarrow> rbt_join l' a (f a b b') r'))"
   by pat_completeness auto
 termination
-  apply (relation "measure (\<lambda>(t1, t2). size t1 + size t2)")
+  apply (relation "measure (\<lambda>(f, t1, t2). size t1 + size t2)")
     apply (auto split: if_splits)
      apply (metis add_leD1 le_imp_less_Suc ord.split_size trans_le_add2)
     apply (metis add_leD1 le_imp_less_Suc ord.split_size trans_le_add1)
@@ -492,21 +496,21 @@ declare inter.simps[simp del]
 lemma rbt_rbtreeify[simp]: "rbt (rbtreeify kvs)"
   by (simp add: rbt_def rbtreeify_def inv1_rbtreeify_g inv2_rbtreeify_g)
 
-lemma rbt_inter: "rbt t1 \<Longrightarrow> rbt t2 \<Longrightarrow> rbt (inter t1 t2)"
-proof(induction t1 t2 rule: inter.induct)
+lemma rbt_inter: "rbt t1 \<Longrightarrow> rbt t2 \<Longrightarrow> rbt (inter f t1 t2)"
+proof(induction f t1 t2 rule: inter.induct)
   case (1 t1 t2)
   thus ?case
     by (auto simp: inter.simps[of t1 t2] inv_rbt_join inv_rbt_join2 split_rbt Let_def rbt_join
         split!: RBT_Impl.rbt.splits RBT_Impl.color.splits unit.splits prod.split if_splits
-        dest!: rbt_Node)
+        option.splits dest!: rbt_Node)
 qed
 
-fun minus :: "'a urbt \<Rightarrow> 'a urbt \<Rightarrow> 'a urbt" where
+fun minus :: "('a, 'b) rbt \<Rightarrow> ('a, 'b) rbt \<Rightarrow> ('a, 'b) rbt" where
   "minus t1 t2 = (if small_rbt t2 then RBT_Impl.fold (\<lambda>k _ t. rbt_delete k t) t2 t1
     else if small_rbt t1 then
       rbtreeify (filter (\<lambda>(k, _). rbt_lookup t2 k = None) (RBT_Impl.entries t1))
     else case t2 of RBT_Impl.Empty \<Rightarrow> t1
-      | RBT_Impl.Branch _ l2 a () r2 \<Rightarrow>
+      | RBT_Impl.Branch _ l2 a b r2 \<Rightarrow>
         case split t1 a of (l1, _, r1) \<Rightarrow> rbt_join2 (minus l1 l2) (minus r1 r2))"
 
 declare minus.simps[simp del]
@@ -544,26 +548,28 @@ context
   fixes comp :: "'a comparator"
 begin
 
-fun split_comp :: "'a urbt \<Rightarrow> 'a \<Rightarrow> 'a urbt \<times> bool \<times> 'a urbt" where
-  "split_comp RBT_Impl.Empty k = (RBT_Impl.Empty, False, RBT_Impl.Empty)"
-| "split_comp (RBT_Impl.Branch _ l a () r) x = (case comp x a of
-    Lt \<Rightarrow> (let (l1,b,l2) = split_comp l x in (l1, b, rbt_join l2 a r))
-  | Gt \<Rightarrow> (let (r1,b,r2) = split_comp r x in (rbt_join l a r1, b, r2))
-  | Eq \<Rightarrow> (l, True, r))"
+fun split_comp :: "('a, 'b) rbt \<Rightarrow> 'a \<Rightarrow> ('a, 'b) rbt \<times> 'b option \<times> ('a, 'b) rbt" where
+  "split_comp RBT_Impl.Empty k = (RBT_Impl.Empty, None, RBT_Impl.Empty)"
+| "split_comp (RBT_Impl.Branch _ l a b r) x = (case comp x a of
+    Lt \<Rightarrow> (case split_comp l x of (l1, \<beta>, l2) \<Rightarrow> (l1, \<beta>, rbt_join l2 a b r))
+  | Gt \<Rightarrow> (case split_comp r x of (r1, \<beta>, r2) \<Rightarrow> (rbt_join l a b r1, \<beta>, r2))
+  | Eq \<Rightarrow> (l, Some b, r))"
 
 lemma split_comp_size: "split_comp t2 a = (l2, b, r2) \<Longrightarrow> size l2 + size r2 \<le> size t2"
   by (induction t2 a arbitrary: l2 b r2 rule: split_comp.induct)
      (auto split: order.splits if_splits prod.splits)
 
-function union_comp :: "'a urbt \<Rightarrow> 'a urbt \<Rightarrow> 'a urbt" where
-  "union_comp t1 t2 = (let (t1, t2) = if flip_rbt t1 t2 then (t2, t1) else (t1, t2) in
-    if small_rbt t1 then RBT_Impl.fold (rbt_comp_insert comp) t1 t2
+function union_comp :: "('a \<Rightarrow> 'b \<Rightarrow> 'b \<Rightarrow> 'b) \<Rightarrow> ('a, 'b) rbt \<Rightarrow> ('a, 'b) rbt \<Rightarrow> ('a, 'b) rbt" where
+  "union_comp f t1 t2 = (let (f, t1, t2) =
+    if flip_rbt t1 t2 then (\<lambda>k v v'. f k v' v, t2, t1) else (f, t1, t2) in
+    if small_rbt t1 then RBT_Impl.fold (rbt_comp_insert_with_key comp f) t1 t2
     else (case t2 of RBT_Impl.Empty \<Rightarrow> t1
-      | RBT_Impl.Branch _ l2 a () r2 \<Rightarrow>
-        case split_comp t1 a of (l1, _, r1) \<Rightarrow> rbt_join (union_comp l1 l2) a (union_comp r1 r2)))"
+      | RBT_Impl.Branch _ l2 a b r2 \<Rightarrow>
+        case split_comp t1 a of (l1, \<beta>, r1) \<Rightarrow>
+          rbt_join (union_comp f l1 l2) a (case \<beta> of None \<Rightarrow> b | Some b' \<Rightarrow> f a b b') (union_comp f r1 r2)))"
   by pat_completeness auto
 termination
-  apply (relation "measure (\<lambda>(t1, t2). size t1 + size t2)")
+  apply (relation "measure (\<lambda>(f,t1, t2). size t1 + size t2)")
     apply (auto split: if_splits)
      apply (metis add_leD1 le_imp_less_Suc split_comp_size trans_le_add2)
     apply (metis add_leD1 le_imp_less_Suc split_comp_size trans_le_add1)
@@ -573,17 +579,19 @@ termination
 
 declare union_comp.simps[simp del]
 
-function inter_comp :: "'a urbt \<Rightarrow> 'a urbt \<Rightarrow> 'a urbt" where
-  "inter_comp t1 t2 = (let (t1, t2) = if flip_rbt t1 t2 then (t2, t1) else (t1, t2) in
+function inter_comp :: "('a \<Rightarrow> 'b \<Rightarrow> 'b \<Rightarrow> 'b) \<Rightarrow> ('a, 'b) rbt \<Rightarrow> ('a, 'b) rbt \<Rightarrow> ('a, 'b) rbt" where
+  "inter_comp f t1 t2 = (let (f, t1, t2) =
+    if flip_rbt t1 t2 then (\<lambda>k v v'. f k v' v, t2, t1) else (f, t1, t2) in
     if small_rbt t1 then
-      rbtreeify (filter (\<lambda>(k, _). rbt_comp_lookup comp t2 k = Some ()) (RBT_Impl.entries t1))
+      rbtreeify (List.map_filter (\<lambda>(k, v). case rbt_comp_lookup comp t2 k of None \<Rightarrow> None
+      | Some v' \<Rightarrow> Some (k, f k v v')) (RBT_Impl.entries t1))
     else case t2 of RBT_Impl.Empty \<Rightarrow> RBT_Impl.Empty
-    | RBT_Impl.Branch _ l2 a () r2 \<Rightarrow>
-      case split_comp t1 a of (l1, ain, r1) \<Rightarrow> let l' = inter_comp l1 l2; r' = inter_comp r1 r2
-      in if ain then rbt_join l' a r' else rbt_join2 l' r')"
+    | RBT_Impl.Branch _ l2 a b r2 \<Rightarrow>
+      case split_comp t1 a of (l1, \<beta>, r1) \<Rightarrow> let l' = inter_comp f l1 l2; r' = inter_comp f r1 r2 in
+      (case \<beta> of None \<Rightarrow> rbt_join2 l' r' | Some b' \<Rightarrow> rbt_join l' a (f a b b') r'))"
   by pat_completeness auto
 termination
-  apply (relation "measure (\<lambda>(t1, t2). size t1 + size t2)")
+  apply (relation "measure (\<lambda>(f, t1, t2). size t1 + size t2)")
     apply (auto split: if_splits)
      apply (metis add_leD1 le_imp_less_Suc split_comp_size trans_le_add2)
     apply (metis add_leD1 le_imp_less_Suc split_comp_size trans_le_add1)
@@ -593,12 +601,12 @@ termination
 
 declare inter_comp.simps[simp del]
 
-fun minus_comp :: "'a urbt \<Rightarrow> 'a urbt \<Rightarrow> 'a urbt" where
+fun minus_comp :: "('a, 'b) rbt \<Rightarrow> ('a, 'b) rbt \<Rightarrow> ('a, 'b) rbt" where
   "minus_comp t1 t2 = (if small_rbt t2 then RBT_Impl.fold (\<lambda>k _ t. rbt_comp_delete comp k t) t2 t1
     else if small_rbt t1 then
       rbtreeify (filter (\<lambda>(k, _). rbt_comp_lookup comp t2 k = None) (RBT_Impl.entries t1))
     else case t2 of RBT_Impl.Empty \<Rightarrow> t1
-      | RBT_Impl.Branch _ l2 a () r2 \<Rightarrow>
+      | RBT_Impl.Branch _ l2 a b r2 \<Rightarrow>
         case split_comp t1 a of (l1, _, r1) \<Rightarrow> rbt_join2 (minus_comp l1 l2) (minus_comp r1 r2))"
 
 declare minus_comp.simps[simp del]
@@ -618,52 +626,48 @@ lemma split_comp: "split_comp c t x = ord.split (lt_of_comp c) t x"
   by (induction t x rule: split_comp.induct[where comp=c])
      (auto simp: ord.split.simps split: order.splits prod.splits dest: anti_sym)
 
-lemma union_comp: "union_comp c t1 t2 = ord.union (lt_of_comp c) t1 t2"
-proof (induction t1 t2 rule: union_comp.induct[where comp=c])
-  case (1 t1 t2)
-  obtain t1' t2' where flip:
-    "(t1', t2') = (if flip_rbt t1 t2 then (t2, t1) else (t1, t2))"
+lemma union_comp: "union_comp c f t1 t2 = ord.union (lt_of_comp c) f t1 t2"
+proof (induction f t1 t2 rule: union_comp.induct[where comp=c])
+  case (1 f t1 t2)
+  obtain f' t1' t2' where flip:
+    "(f', t1', t2') = (if flip_rbt t1 t2 then (\<lambda>k v v'. f k v' v, t2, t1) else (f, t1, t2))"
     by fastforce
   show ?case
   proof (cases t2')
-    case (Branch _ l2 a u r2)
+    case (Branch _ l2 a b r2)
     have t1_not_Empty: "t2' \<noteq> RBT_Impl.Empty"
       by (auto simp: Branch)
-    have u_def: "u = ()"
-      by auto
-    obtain l1 b r1 where split: "split_comp c t1' a = (l1, b, r1)"
+    obtain l1 \<beta> r1 where split: "split_comp c t1' a = (l1, \<beta>, r1)"
       by (cases "split_comp c t1' a") auto
     show ?thesis
-      using 1[OF flip refl _ Branch]
-      unfolding union_comp.simps[of _ t1] ord.union.simps[of _ t1] flip[symmetric]
-      by (auto simp: Branch split split_comp[symmetric] rbt_comp_insert[OF c]
+      using 1[OF flip refl _ _ Branch]
+      unfolding union_comp.simps[of _ _ t1] ord.union.simps[of _ _ t1] flip[symmetric]
+      by (auto simp: Branch split split_comp[symmetric] rbt_comp_insert_with_key[OF c]
           split: unit.splits prod.splits)
-  qed (auto simp: union_comp.simps[of _ t1] ord.union.simps[of _ t1] flip[symmetric]
-       rbt_comp_insert[OF c] split_comp[symmetric])
+  qed (auto simp: union_comp.simps[of _ _ t1] ord.union.simps[of _ _ t1] flip[symmetric]
+       rbt_comp_insert_with_key[OF c] split_comp[symmetric])
 qed
 
-lemma inter_comp: "inter_comp c t1 t2 = ord.inter (lt_of_comp c) t1 t2"
-proof (induction t1 t2 rule: inter_comp.induct[where comp=c])
-  case (1 t1 t2)
-  obtain t1' t2' where flip:
-    "(t1', t2') = (if flip_rbt t1 t2 then (t2, t1) else (t1, t2))"
+lemma inter_comp: "inter_comp c f t1 t2 = ord.inter (lt_of_comp c) f t1 t2"
+proof (induction f t1 t2 rule: inter_comp.induct[where comp=c])
+  case (1 f t1 t2)
+  obtain f' t1' t2' where flip:
+    "(f', t1', t2') = (if flip_rbt t1 t2 then (\<lambda>k v v'. f k v' v, t2, t1) else (f, t1, t2))"
     by fastforce
   show ?case
   proof (cases t2')
-    case (Branch _ l2 a u r2)
+    case (Branch _ l2 a b r2)
     have t1_not_Empty: "t2' \<noteq> RBT_Impl.Empty"
       by (auto simp: Branch)
-    have u_def: "u = ()"
-      by auto
-    obtain l1 b r1 where split: "split_comp c t1' a = (l1, b, r1)"
+    obtain l1 \<beta> r1 where split: "split_comp c t1' a = (l1, \<beta>, r1)"
       by (cases "split_comp c t1' a") auto
     show ?thesis
-      using 1[OF flip refl _ Branch]
-      unfolding inter_comp.simps[of _ t1] ord.inter.simps[of _ t1] flip[symmetric]
-      by (auto simp: Branch split split_comp[symmetric] rbt_comp_insert[OF c] rbt_comp_lookup[OF c]
+      using 1[OF flip refl _ _ Branch]
+      unfolding inter_comp.simps[of _ _ t1] ord.inter.simps[of _ _ t1] flip[symmetric]
+      by (auto simp: Branch split split_comp[symmetric] rbt_comp_lookup[OF c]
           split: unit.splits prod.splits)
-  qed (auto simp: inter_comp.simps[of _ t1] ord.inter.simps[of _ t1] flip[symmetric]
-       rbt_comp_insert[OF c] rbt_comp_lookup[OF c] split_comp[symmetric])
+  qed (auto simp: inter_comp.simps[of _ _ t1] ord.inter.simps[of _ _ t1] flip[symmetric]
+       rbt_comp_lookup[OF c] split_comp[symmetric])
 qed
 
 lemma minus_comp: "minus_comp c t1 t2 = ord.minus (lt_of_comp c) t1 t2"
@@ -674,9 +678,7 @@ proof (induction t1 t2 rule: minus_comp.induct[where comp=c])
     case (Branch _ l2 a u r2)
     have t2_not_Empty: "t2 \<noteq> RBT_Impl.Empty"
       by (auto simp: Branch)
-    have u_def: "u = ()"
-      by auto
-    obtain l1 b r1 where split: "split_comp c t1 a = (l1, b, r1)"
+    obtain l1 \<beta> r1 where split: "split_comp c t1 a = (l1, \<beta>, r1)"
       by (cases "split_comp c t1 a") auto
     show ?thesis
       using 1[OF _ _ Branch]
@@ -692,51 +694,51 @@ end
 context linorder begin
 
 lemma rbt_sorted_baliL:
-  "\<lbrakk>rbt_sorted l; rbt_sorted r; l |\<guillemotleft> a; a \<guillemotleft>| r\<rbrakk> \<Longrightarrow> rbt_sorted (baliL l a r)"
+  "\<lbrakk>rbt_sorted l; rbt_sorted r; l |\<guillemotleft> a; a \<guillemotleft>| r\<rbrakk> \<Longrightarrow> rbt_sorted (baliL l a b r)"
   using rbt_greater_trans rbt_less_trans
-  apply (cases "(l,a,r)" rule: baliL.cases)
+  apply (cases "(l,a,b,r)" rule: baliL.cases)
             apply (auto simp: rbt_sorted_def)
    apply blast+
   done
 
 lemma rbt_sorted_baliR:
-  "\<lbrakk>rbt_sorted l; rbt_sorted r; l |\<guillemotleft> a; a \<guillemotleft>| r\<rbrakk> \<Longrightarrow> rbt_sorted (baliR l a r)"
+  "\<lbrakk>rbt_sorted l; rbt_sorted r; l |\<guillemotleft> a; a \<guillemotleft>| r\<rbrakk> \<Longrightarrow> rbt_sorted (baliR l a b r)"
   using rbt_greater_trans rbt_less_trans
-  apply (cases "(l,a,r)" rule: baliR.cases)
+  apply (cases "(l,a,b,r)" rule: baliR.cases)
             apply (auto simp: rbt_sorted_def)
     apply blast+
   done
 
 lemma rbt_sorted_rbt_joinL:
-  "\<lbrakk>rbt_sorted (RBT_Impl.Branch c l a () r); bheight l \<le> bheight r\<rbrakk>
-  \<Longrightarrow> rbt_sorted (rbt_joinL l a r)"
-proof (induction l a r arbitrary: c rule: rbt_joinL.induct)
-  case (1 l a r)
+  "\<lbrakk>rbt_sorted (RBT_Impl.Branch c l a b r); bheight l \<le> bheight r\<rbrakk>
+  \<Longrightarrow> rbt_sorted (rbt_joinL l a b r)"
+proof (induction l a b r arbitrary: c rule: rbt_joinL.induct)
+  case (1 l a b r)
   thus ?case
-    by (auto simp: set_baliL rbt_joinL.simps[of l a r] set_rbt_joinL rbt_less_prop
+    by (auto simp: set_baliL rbt_joinL.simps[of l a b r] set_rbt_joinL rbt_less_prop
         intro!: rbt_sorted_baliL split!: RBT_Impl.rbt.splits RBT_Impl.color.splits unit.splits)
 qed
 
 lemma rbt_sorted_rbt_joinR:
   "\<lbrakk>rbt_sorted l; rbt_sorted r; l |\<guillemotleft> a; a \<guillemotleft>| r\<rbrakk>
-  \<Longrightarrow> rbt_sorted (rbt_joinR l a r)"
-proof (induction l a r rule: rbt_joinR.induct)
-  case (1 l a r)
+  \<Longrightarrow> rbt_sorted (rbt_joinR l a b r)"
+proof (induction l a b r rule: rbt_joinR.induct)
+  case (1 l a b r)
   thus ?case
-    by (auto simp: set_baliR rbt_joinR.simps[of l a r] set_rbt_joinR rbt_greater_prop
+    by (auto simp: set_baliR rbt_joinR.simps[of l a b r] set_rbt_joinR rbt_greater_prop
         intro!: rbt_sorted_baliR split!: RBT_Impl.rbt.splits RBT_Impl.color.splits unit.splits)
 qed
 
 lemma rbt_sorted_paint: "rbt_sorted (paint c t) = rbt_sorted t"
   by (cases t) auto
 
-lemma rbt_sorted_rbt_join: "rbt_sorted (RBT_Impl.Branch c l a () r) \<Longrightarrow>
-  rbt_sorted (rbt_join l a r)"
+lemma rbt_sorted_rbt_join: "rbt_sorted (RBT_Impl.Branch c l a b r) \<Longrightarrow>
+  rbt_sorted (rbt_join l a b r)"
   by (auto simp: rbt_sorted_paint rbt_sorted_rbt_joinL rbt_sorted_rbt_joinR rbt_join_def)
 
 lemma split_min_rbt_sorted:
-  "\<lbrakk> split_min t = (m,t');  rbt_sorted t;  t \<noteq> RBT_Impl.Empty \<rbrakk> \<Longrightarrow>
-  rbt_sorted t' \<and> (\<forall>x \<in> set (RBT_Impl.keys t'). m < x)"
+  "\<lbrakk> split_min t = (a,b,t');  rbt_sorted t;  t \<noteq> RBT_Impl.Empty \<rbrakk> \<Longrightarrow>
+  rbt_sorted t' \<and> (\<forall>x \<in> set (RBT_Impl.keys t'). a < x)"
   by (induction t arbitrary: t')
      (fastforce simp: split_min_set rbt_sorted_rbt_join set_rbt_join rbt_less_prop rbt_greater_prop
       split: if_splits prod.splits)+
@@ -747,23 +749,28 @@ lemma rbt_sorted_rbt_join2:
   by (simp add: rbt_join2_def rbt_sorted_rbt_join split_min_set split_min_rbt_sorted set_rbt_join
       rbt_greater_prop rbt_less_prop split: prod.split)
 
-lemma split: "split t x = (l,xin,r) \<Longrightarrow> rbt_sorted t \<Longrightarrow>
+lemma split: "split t x = (l,\<beta>,r) \<Longrightarrow> rbt_sorted t \<Longrightarrow>
   set (RBT_Impl.keys l) = {a \<in> set (RBT_Impl.keys t). a < x} \<and>
   set (RBT_Impl.keys r) = {a \<in> set (RBT_Impl.keys t). x < a} \<and>
-  (xin = (x \<in> set (RBT_Impl.keys t))) \<and> rbt_sorted l \<and> rbt_sorted r"
-  by (induction t arbitrary: l xin r)
+  rbt_sorted l \<and> rbt_sorted r"
+  by (induction t arbitrary: l r)
+     (force simp: Let_def set_rbt_join rbt_greater_prop rbt_less_prop
+      split: if_splits prod.splits intro!: rbt_sorted_rbt_join)+
+
+lemma split_lookup: "split t x = (l,\<beta>,r) \<Longrightarrow> rbt_sorted t \<Longrightarrow> \<beta> = rbt_lookup t x"
+  by (induction t arbitrary: l r)
      (force simp: Let_def set_rbt_join rbt_greater_prop rbt_less_prop
       split: if_splits prod.splits intro!: rbt_sorted_rbt_join)+
 
 lemma keys_paint'[simp]: "RBT_Impl.keys (RBT_Impl.paint c t) = RBT_Impl.keys t"
   by (cases t) auto
 
-lemma [simp]: "set (RBT_Impl.keys (rbt_insert x y t2)) = {x} \<union> set (RBT_Impl.keys t2)"
-  by (auto simp: rbt_insert_def rbt_insert_with_key_def keys_ins)
+lemma [simp]: "set (RBT_Impl.keys (rbt_insert_with_key f a b t2)) = {a} \<union> set (RBT_Impl.keys t2)"
+  by (auto simp: rbt_insert_with_key_def keys_ins)
 
 lemma set_tree_fold_insert:
   assumes "rbt_sorted t2"
-  shows "set (RBT_Impl.keys (RBT_Impl.fold rbt_insert t1 t2)) =
+  shows "set (RBT_Impl.keys (RBT_Impl.fold (rbt_insert_with_key f) t1 t2)) =
     set (RBT_Impl.keys t1) \<union> set (RBT_Impl.keys t2)"
 proof -
   define xs where "xs = RBT_Impl.entries t1"
@@ -771,16 +778,21 @@ proof -
     by (auto simp: xs_def RBT_Impl.keys_def)
   from assms show ?thesis
     unfolding RBT_Impl.fold_def xs_def[symmetric] keys_t1
-    by (induct xs rule: rev_induct) (auto simp: rev_image_eqI)
+    by (induction xs rule: rev_induct) (auto simp: rev_image_eqI)
 qed
 
+lemma rbt_sorted_fold_insertwk:
+  "rbt_sorted t \<Longrightarrow> rbt_sorted (RBT_Impl.fold (rbt_insert_with_key f) t' t)"
+  by (induct t' arbitrary: t)
+     (simp_all add: rbt_insertwk_rbt_sorted)
+
 lemma rbt_sorted_union: "rbt_sorted t1 \<Longrightarrow> rbt_sorted t2 \<Longrightarrow>
-  set (RBT_Impl.keys (union t1 t2)) = set (RBT_Impl.keys t1) \<union> set (RBT_Impl.keys t2) \<and>
-  rbt_sorted (union t1 t2)"
-proof(induction t1 t2 rule: union.induct)
-  case (1 t1 t2)
-  obtain t1' t2' where flip:
-    "(t1', t2') = (if flip_rbt t1 t2 then (t2, t1) else (t1, t2))"
+  set (RBT_Impl.keys (union f t1 t2)) = set (RBT_Impl.keys t1) \<union> set (RBT_Impl.keys t2) \<and>
+  rbt_sorted (union f t1 t2)"
+proof(induction f t1 t2 rule: union.induct)
+  case (1 f t1 t2)
+  obtain f' t1' t2' where flip:
+    "(f', t1', t2') = (if flip_rbt t1 t2 then (\<lambda>k v v'. f k v' v, t2, t1) else (f, t1, t2))"
     by fastforce
   have set_flip: "set (RBT_Impl.keys t1) \<union> set (RBT_Impl.keys t2) =
       set (RBT_Impl.keys t1') \<union> set (RBT_Impl.keys t2')"
@@ -791,61 +803,80 @@ proof(induction t1 t2 rule: union.induct)
     by (auto split: if_splits)
   then show ?case
   proof (cases t2')
-    case (Branch _ l2 a u r2)
-    obtain l1 b r1 where split_t1': "split t1' a = (l1, b, r1)"
+    case (Branch _ l2 a b r2)
+    obtain l1 \<beta> r1 where split_t1': "split t1' a = (l1, \<beta>, r1)"
       by (cases "split t1' a") auto
     have rbt_sort: "rbt_sorted l2" "rbt_sorted r2"
       using 1(3,4) flip
       by (auto simp: Branch split: if_splits)
     note split_t1'_prop = split[OF split_t1' rbt_sorted'(1)]
     have union_l1_l2: "\<not>small_rbt t1' \<Longrightarrow>
-      set (RBT_Impl.keys (union l1 l2)) = set (RBT_Impl.keys l1) \<union> set (RBT_Impl.keys l2) \<and>
-      rbt_sorted (union l1 l2)"
-      using 1(1)[OF flip _ _ Branch _ split_t1'[symmetric]] rbt_sort split_t1'_prop
+      set (RBT_Impl.keys (union f' l1 l2)) = set (RBT_Impl.keys l1) \<union> set (RBT_Impl.keys l2) \<and>
+      rbt_sorted (union f' l1 l2)"
+      using 1(1)[OF flip refl refl _ Branch split_t1'[symmetric]] rbt_sort split_t1'_prop
       by auto
     have union_r1_r2: "\<not>small_rbt t1' \<Longrightarrow>
-      set (RBT_Impl.keys (union r1 r2)) = set (RBT_Impl.keys r1) \<union> set (RBT_Impl.keys r2) \<and>
-      rbt_sorted (union r1 r2)"
-      using 1(2)[OF flip _ _ Branch _ split_t1'[symmetric]] rbt_sort split_t1'_prop
+      set (RBT_Impl.keys (union f' r1 r2)) = set (RBT_Impl.keys r1) \<union> set (RBT_Impl.keys r2) \<and>
+      rbt_sorted (union f' r1 r2)"
+      using 1(2)[OF flip refl refl _ Branch split_t1'[symmetric]] rbt_sort split_t1'_prop
       by auto
-    have "set (RBT_Impl.keys (union t1 t2)) = set (RBT_Impl.keys t1) \<union> set (RBT_Impl.keys t2)"
+    have "set (RBT_Impl.keys (union f t1 t2)) = set (RBT_Impl.keys t1) \<union> set (RBT_Impl.keys t2)"
       using rbt_sorted' union_l1_l2 union_r1_r2 split_t1'_prop
-      unfolding set_flip
-      by (auto 0 0 simp: union.simps[of t1] flip[symmetric] set_tree_fold_insert)
-         (auto simp: Branch split_t1' set_rbt_join split!: unit.splits if_splits)
-    moreover have "rbt_sorted (union t1 t2)"
+      unfolding set_flip union.simps[of _ t1] flip[symmetric]
+      by (auto simp: set_tree_fold_insert Branch split_t1' set_rbt_join
+          split!: unit.splits if_splits option.splits)
+    moreover have "rbt_sorted (union f t1 t2)"
       using rbt_sorted' 1(3,4) union_l1_l2 union_r1_r2 split_t1'_prop
-      by (auto 0 0 simp: union.simps[of t1] flip[symmetric] rbt_sorted_fold_insert)
-         (auto simp: Branch split_t1' rbt_less_prop rbt_greater_prop intro!: rbt_sorted_rbt_join
-          split!: unit.splits if_splits)
+      unfolding set_flip union.simps[of _ t1] flip[symmetric]
+      by (auto simp: rbt_sorted_fold_insertwk Branch split_t1' rbt_less_prop rbt_greater_prop
+          intro!: rbt_sorted_rbt_join
+          split!: unit.splits if_splits option.splits)
     ultimately show ?thesis
       by auto
-  qed (auto simp: set_flip union.simps[of t1] flip[symmetric] set_tree_fold_insert
-       intro!: rbt_sorted_fold_insert)
+  qed (auto simp: set_flip union.simps[of _ t1] flip[symmetric] set_tree_fold_insert
+       intro!: rbt_sorted_fold_insertwk)
 qed
 
-lemma rbt_sorted_rbtreeify:
-  "rbt_sorted t \<Longrightarrow> rbt_sorted (rbtreeify (filter P (RBT_Impl.entries t)))"
-  using distinct_map_filterI distinct_entries rbt_sorted_entries rbt_sorted_rbtreeify sorted_filter
-  by blast
+lemma rbt_sorted_rbtreeify_map_filter:
+  assumes "rbt_sorted t"
+  shows "rbt_sorted (rbtreeify (List.map_filter
+    (\<lambda>(k, v). case rbt_lookup t2 k of None \<Rightarrow> None
+    | Some v' \<Rightarrow> Some (k, f k v v')) (RBT_Impl.entries t)))"
+proof -
+  have unfold: "map fst (List.map_filter (\<lambda>(k, v). case P k of None \<Rightarrow> None
+    | Some v' \<Rightarrow> Some (k, f k v v')) xs) =
+    filter (\<lambda>k. case P k of None \<Rightarrow> False | _ \<Rightarrow> True) (map fst xs)"
+    for P xs
+    by (induction xs) (auto simp: List.map_filter_def split: option.splits)
+  show ?thesis
+    using rbt_sorted_entries[OF assms] distinct_entries[OF assms] sorted_filter[of id]
+    by (auto simp: unfold intro!: rbt_sorted_rbtreeify)
+qed
 
-lemma rbtreeify_keys_Some:
-  assumes "rbt_sorted t1"
-  shows "set (RBT_Impl.keys (rbtreeify (filter (\<lambda>(k, _). rbt_lookup t1 k = Some ())
-  (RBT_Impl.entries t2)))) = set (RBT_Impl.keys t1) \<inter> set (RBT_Impl.keys t2)"
-  apply (auto simp: RBT_Impl.keys_def map_of_entries[OF assms, symmetric])
-   apply (metis map_of_eq_None_iff not_None_eq)
-  using image_iff weak_map_of_SomeI
-  apply fastforce
+lemma rbtreeify_keys_map_filter: "rbt_sorted t2 \<Longrightarrow>
+  set (RBT_Impl.keys (rbtreeify (List.map_filter (\<lambda>(k, v). case rbt_lookup t2 k of None \<Rightarrow> None
+    | Some v' \<Rightarrow> Some (k, f k v v')) (RBT_Impl.entries t1)))) =
+  set (RBT_Impl.keys t1) \<inter> set (RBT_Impl.keys t2)"
+  apply (auto simp: RBT_Impl.keys_def List.map_filter_def split: option.splits)
+    apply force
+   apply (metis local.map_of_entries map_of_eq_None_iff option.distinct(1))
+  apply (smt image_iff local.map_of_entries local.rbt_lookup_in_tree mem_Collect_eq
+      option.case(2) option.collapse option.distinct(1) option.simps(1) prod.sel(1) prod.simps(2))
   done
 
+lemma rbt_lookup_iff_keys:
+  "rbt_sorted t \<Longrightarrow> rbt_lookup t k = None \<longleftrightarrow> k \<notin> set (RBT_Impl.keys t)"
+  "rbt_sorted t \<Longrightarrow> (\<exists>v. rbt_lookup t k = Some v) \<longleftrightarrow> k \<in> set (RBT_Impl.keys t)"
+  using entry_in_tree_keys rbt_lookup_keys[of t]
+  by (fastforce simp: RBT_Impl.keys_def dom_def)+
+
 lemma rbt_sorted_inter: "rbt_sorted t1 \<Longrightarrow> rbt_sorted t2 \<Longrightarrow>
-  set (RBT_Impl.keys (inter t1 t2)) = set (RBT_Impl.keys t1) \<inter> set (RBT_Impl.keys t2) \<and>
-  rbt_sorted (inter t1 t2)"
-proof(induction t1 t2 rule: inter.induct)
-  case (1 t1 t2)
-  obtain t1' t2' where flip:
-    "(t1', t2') = (if flip_rbt t1 t2 then (t2, t1) else (t1, t2))"
+  set (RBT_Impl.keys (inter f t1 t2)) = set (RBT_Impl.keys t1) \<inter> set (RBT_Impl.keys t2) \<and>
+  rbt_sorted (inter f t1 t2)"
+proof(induction f t1 t2 rule: inter.induct)
+  case (1 f t1 t2)
+  obtain f' t1' t2' where flip:
+    "(f', t1', t2') = (if flip_rbt t1 t2 then (\<lambda>k v v'. f k v' v, t2, t1) else (f, t1, t2))"
     by fastforce
   have set_flip: "set (RBT_Impl.keys t1) \<inter> set (RBT_Impl.keys t2) =
     set (RBT_Impl.keys t1') \<inter> set (RBT_Impl.keys t2')"
@@ -861,21 +892,21 @@ proof(induction t1 t2 rule: inter.induct)
       set (RBT_Impl.keys t1') \<inter> set (RBT_Impl.keys t2')"
       using flip
       by (auto split: if_splits)
-    obtain l1 b r1 where sp: "split t1' a = (l1, b, r1)"
+    obtain l1 \<beta> r1 where sp: "split t1' a = (l1, \<beta>, r1)"
       by (cases "split t1' a") auto
     have rbt_sort: "rbt_sorted l2" "rbt_sorted r2"
       using 1(3,4) flip
       by (auto split: if_splits)
     note split_t1'_prop = split[OF sp rbt_sorted'(1)]
     have inter_l1_l2: "\<not>small_rbt t1' \<Longrightarrow>
-      set (RBT_Impl.keys (inter l1 l2)) = set (RBT_Impl.keys l1) \<inter> set (RBT_Impl.keys l2) \<and>
-      rbt_sorted (inter l1 l2)"
-      using 1(1)[OF flip _ _ Branch _ sp[symmetric]] rbt_sort split_t1'_prop
+      set (RBT_Impl.keys (inter f' l1 l2)) = set (RBT_Impl.keys l1) \<inter> set (RBT_Impl.keys l2) \<and>
+      rbt_sorted (inter f' l1 l2)"
+      using 1(1)[OF flip refl refl _ Branch sp[symmetric]] rbt_sort split_t1'_prop
       by auto
     have inter_r1_r2: "\<not>small_rbt t1' \<Longrightarrow>
-      set (RBT_Impl.keys (inter r1 r2)) = set (RBT_Impl.keys r1) \<inter> set (RBT_Impl.keys r2) \<and>
-      rbt_sorted (inter r1 r2)"
-      using 1(2)[OF flip _ _ Branch _ sp[symmetric]] rbt_sort split_t1'_prop
+      set (RBT_Impl.keys (inter f' r1 r2)) = set (RBT_Impl.keys r1) \<inter> set (RBT_Impl.keys r2) \<and>
+      rbt_sorted (inter f' r1 r2)"
+      using 1(2)[OF flip refl refl _ Branch sp[symmetric]] rbt_sort split_t1'_prop
       by auto
     {
       assume not_small: "\<not>small_rbt t1'"
@@ -885,52 +916,52 @@ proof(induction t1 t2 rule: inter.induct)
         by (auto simp: rbt_less_prop rbt_greater_prop)
       let ?L1 = "set (RBT_Impl.keys l1)"
       let ?R1 = "set (RBT_Impl.keys r1)"
-      let ?K = "if b then {a} else {}"
+      let ?K = "case \<beta> of None \<Rightarrow> {} | _ \<Rightarrow> {a}"
       have t2: "set (RBT_Impl.keys t1') = ?L1 \<union> ?R1 \<union> ?K" and
         **: "?L1 \<inter> ?R1 = {}" "a \<notin> ?L1 \<union> ?R1" "?L2 \<inter> ?R1 = {}" "?L1 \<inter> ?R2 = {}"
-        using split[OF sp] less_linear \<open>rbt_sorted t1'\<close> \<open>rbt_sorted t2'\<close>
-        by (auto simp: rbt_less_prop rbt_greater_prop)
+        using split[OF sp] split_lookup[OF sp] rbt_lookup_iff_keys[of t1'] less_linear rbt_sorted'
+        by (auto simp: rbt_less_prop rbt_greater_prop split: option.splits)
       have "set (RBT_Impl.keys t1') \<inter> set (RBT_Impl.keys t2') =
         (?L2 \<union> ?R2 \<union> {a}) \<inter> (?L1 \<union> ?R1 \<union> ?K)"
         by (auto simp add: t2)
       also have "\<dots> = (?L1 \<inter> ?L2) \<union> (?R1 \<inter> ?R2) \<union> ?K"
-        using * ** by auto
-      also have "\<dots> = set (RBT_Impl.keys (inter t1 t2))"
+        using * **
+        by (auto split: option.splits)
+      also have "\<dots> = set (RBT_Impl.keys (inter f t1 t2))"
         using inter_l1_l2[OF not_small] inter_r1_r2[OF not_small]
-        by (auto simp: inter.simps[of t1] flip[symmetric] not_small sp set_rbt_join
-            split: unit.splits)
-      finally have "set (RBT_Impl.keys (inter t1 t2)) =
+        by (auto simp: inter.simps[of _ t1] flip[symmetric] not_small sp set_rbt_join
+            split: unit.splits option.splits)
+      finally have "set (RBT_Impl.keys (inter f t1 t2)) =
       set (RBT_Impl.keys t1) \<inter> set (RBT_Impl.keys t2)"
         unfolding set_flip
         by auto
     }
-    moreover have "small_rbt t1' \<Longrightarrow> set (RBT_Impl.keys (inter t1 t2)) =
-      set (RBT_Impl.keys (rbtreeify (filter (\<lambda>(k, _). rbt_lookup t2' k = Some ())
-      (RBT_Impl.entries t1'))))"
-      by (auto simp: inter.simps[of t1] flip[symmetric])
-    ultimately have "set (RBT_Impl.keys (ord_class.inter t1 t2)) =
+    moreover have "small_rbt t1' \<Longrightarrow> set (RBT_Impl.keys (inter f t1 t2)) =
+      set (RBT_Impl.keys (rbtreeify (List.map_filter (\<lambda>(k, v). case rbt_lookup t2' k of None \<Rightarrow> None
+    | Some v' \<Rightarrow> Some (k, f' k v v')) (RBT_Impl.entries t1'))))"
+      by (auto simp: inter.simps[of _ t1] flip[symmetric])
+    ultimately have "set (RBT_Impl.keys (ord_class.inter f t1 t2)) =
       set (RBT_Impl.keys t1) \<inter> set (RBT_Impl.keys t2)"
       using flip
-      unfolding rbtreeify_keys_Some[OF rbt_sorted'(2)] set_flip
+      unfolding rbtreeify_keys_map_filter[OF rbt_sorted'(2)] set_flip
       by auto
-    moreover have "rbt_sorted (inter t1 t2)"
+    moreover have "rbt_sorted (inter f t1 t2)"
       using rbt_sorted'(1) rbt_sort 1(3,4) inter_l1_l2 inter_r1_r2 split_t1'_prop
-      by (auto 0 0 simp: inter.simps[of t1] flip[symmetric] sp rbt_less_prop rbt_greater_prop
-          intro!: rbt_sorted_rbtreeify rbt_sorted_rbt_join rbt_sorted_rbt_join2
-          split!: unit.splits if_splits)
-         (meson local.order.strict_trans)
+      by (auto simp: inter.simps[of _ t1] flip[symmetric] sp rbt_less_prop rbt_greater_prop Let_def
+          intro!: rbt_sorted_rbtreeify_map_filter rbt_sorted_rbt_join rbt_sorted_rbt_join2
+          split!: unit.splits if_splits option.splits)
     ultimately show ?thesis
       by auto
-  qed (auto simp: rbtreeify_def set_flip inter.simps[of t1] flip[symmetric])
+  qed (auto simp: rbtreeify_def set_flip inter.simps[of _ t1] flip[symmetric] List.map_filter_def)
 qed
 
 lemma [simp]: "RBT_Impl.entries (RBT_Impl.paint c t) = RBT_Impl.entries t"
   by (cases t) auto
 
 lemma [simp]: "rbt t \<Longrightarrow> rbt_sorted t \<Longrightarrow>
-  set (RBT_Impl.keys (rbt_delete x t)) = set (RBT_Impl.keys t) - {x}"
-  using rbt_del_in_tree image_iff
-  by (fastforce simp: rbt_def RBT_Impl.keys_def rbt_delete_def)
+  set (RBT_Impl.keys (rbt_delete a t)) = set (RBT_Impl.keys t) - {a}"
+  using rbt_del_in_tree[of t]
+  by (auto simp: rbt_def RBT_Impl.keys_def rbt_delete_def)
 
 lemma [simp]: "rbt_sorted t \<Longrightarrow> rbt_sorted (rbt_delete x t)"
   by (auto simp: rbt_delete_def rbt_del_rbt_sorted)
@@ -968,6 +999,11 @@ lemma rbtreeify_keys_None:
   apply (smt fst_conv image_iff map_of_eq_None_iff mem_Collect_eq)
   done
 
+lemma rbt_sorted_rbtreeify_filter:
+  "rbt_sorted t \<Longrightarrow> rbt_sorted (rbtreeify (filter P (RBT_Impl.entries t)))"
+  using distinct_map_filterI distinct_entries rbt_sorted_entries rbt_sorted_rbtreeify sorted_filter
+  by blast
+
 lemma rbt_sorted_minus:
   "rbt t1 \<Longrightarrow> rbt_sorted t1 \<Longrightarrow> rbt_sorted t2 \<Longrightarrow>
   set (RBT_Impl.keys (minus t1 t2)) = set (RBT_Impl.keys t1) - set (RBT_Impl.keys t2) \<and>
@@ -978,33 +1014,33 @@ proof(induction t1 t2 rule: minus.induct)
   proof (cases t2)
     case Empty
     show ?thesis
-      using 1(4,5)
+      using 1(4,5) rbt_sorted_entries distinct_entries
       by (auto simp: minus.simps rbtreeify_keys_None intro!: rbt_sorted_rbtreeify)
          (auto simp: Empty)
   next
     case [simp]: (Branch _ l2 a _ r2)
     let ?L2 = "set (RBT_Impl.keys l2)" let ?R2 = "set (RBT_Impl.keys r2)"
-    obtain l1 ain r1 where sp: "split t1 a = (l1,ain,r1)" using prod_cases3 by blast
+    obtain l1 \<beta> r1 where sp: "split t1 a = (l1,\<beta>,r1)" using prod_cases3 by blast
     let ?L1 = "set (RBT_Impl.keys l1)"
     let ?R1 = "set (RBT_Impl.keys r1)"
-    let ?K = "if ain then {a} else {}"
+    let ?K = "case \<beta> of None \<Rightarrow> {} | _ \<Rightarrow> {a}"
     have rbt_l1_r1: "rbt l1" "rbt r1"
       using split_rbt[OF sp 1(3)]
       by auto
     have t1: "set (RBT_Impl.keys t1) = ?L1 \<union> ?R1 \<union> ?K" and
       **: "a \<notin> ?L1 \<union> ?R1" "?L1 \<inter> ?R2 = {}" "?L2 \<inter> ?R1 = {}"
-      using split[OF sp] less_linear \<open>rbt_sorted t1\<close> \<open>rbt_sorted t2\<close>
-      by (auto simp: rbt_less_prop rbt_greater_prop)
+      using split[OF sp] split_lookup[OF sp] rbt_lookup_iff_keys[of t1] less_linear 1(4,5)
+      by (auto simp: rbt_less_prop rbt_greater_prop split: option.splits)
     have IHl: "\<not> small_rbt t1 \<Longrightarrow> \<not>small_rbt t2 \<Longrightarrow> set (RBT_Impl.keys (minus l1 l2)) =
       set (RBT_Impl.keys l1) - set (RBT_Impl.keys l2) \<and> rbt_sorted (minus l1 l2)"
-      using "1.IH"(1)[OF _ _ _ _ sp[symmetric]] "1.prems"(1,2,3) split[OF sp] rbt_l1_r1 by simp
+      using "1.IH"(1)[OF _ _ _ sp[symmetric]] "1.prems"(1,2,3) split[OF sp] rbt_l1_r1 by simp
     have IHr: "\<not> small_rbt t1 \<Longrightarrow> \<not>small_rbt t2 \<Longrightarrow> set (RBT_Impl.keys (minus r1 r2)) =
       set (RBT_Impl.keys r1) - set (RBT_Impl.keys r2) \<and> rbt_sorted (minus r1 r2)"
-      using "1.IH"(2)[OF _ _ _ _ sp[symmetric]] "1.prems"(1,2,3) split[OF sp] rbt_l1_r1 by simp
+      using "1.IH"(2)[OF _ _ _ sp[symmetric]] "1.prems"(1,2,3) split[OF sp] rbt_l1_r1 by simp
     {
       assume IH: "\<not>small_rbt t1" "\<not>small_rbt t2"
       have "set (RBT_Impl.keys t1) - set (RBT_Impl.keys t2) = (?L1 \<union> ?R1) - (?L2 \<union> ?R2  \<union> {a})"
-        by (simp add: t1)
+        by (simp add: t1 split: option.splits)
       also have "\<dots> = (?L1 - ?L2) \<union> (?R1 - ?R2)"
         using ** by auto
       also have "\<dots> = set (RBT_Impl.keys (minus t1 t2))"
@@ -1021,14 +1057,14 @@ proof(induction t1 t2 rule: minus.induct)
     moreover have "rbt_sorted (minus t1 t2)"
       using 1(3,4,5) IHl IHr split[OF sp 1(4)]
       by (auto simp: minus.simps[of t1] sp rbt_less_prop rbt_greater_prop rbt_sorted_fold_delete
-          intro!: rbt_sorted_rbtreeify rbt_sorted_rbt_join rbt_sorted_rbt_join2
+          intro!: rbt_sorted_rbtreeify_filter rbt_sorted_rbt_join rbt_sorted_rbt_join2
           split!: unit.splits if_splits)
     ultimately show ?thesis
       by auto
   qed
 qed
 
-definition is_rbt_aux :: "'a urbt \<Rightarrow> bool" where
+definition is_rbt_aux :: "('a, 'b) rbt \<Rightarrow> bool" where
   "is_rbt_aux t \<longleftrightarrow> inv1 t \<and> inv2 t \<and> rbt_sorted t"
 
 lemma is_rbt_aux_prop: "is_rbt_aux t \<longleftrightarrow> rbt t \<and> rbt_sorted t"
@@ -1037,11 +1073,11 @@ lemma is_rbt_aux_prop: "is_rbt_aux t \<longleftrightarrow> rbt t \<and> rbt_sort
 lemma is_rbt_prop: "is_rbt t \<longleftrightarrow> is_rbt_aux t \<and> color_of t = RBT_Impl.B"
   by (auto simp: is_rbt_def is_rbt_aux_def)
 
-lemma is_rbt_aux_union: "\<lbrakk> is_rbt_aux t1; is_rbt_aux t2 \<rbrakk> \<Longrightarrow> is_rbt_aux (union t1 t2)"
+lemma is_rbt_aux_union: "\<lbrakk> is_rbt_aux t1; is_rbt_aux t2 \<rbrakk> \<Longrightarrow> is_rbt_aux (union f t1 t2)"
   using rbt_sorted_union rbt_union
   by (auto simp: is_rbt_aux_prop)
 
-lemma is_rbt_aux_inter: "\<lbrakk> is_rbt_aux t1; is_rbt_aux t2 \<rbrakk> \<Longrightarrow> is_rbt_aux (inter t1 t2)"
+lemma is_rbt_aux_inter: "\<lbrakk> is_rbt_aux t1; is_rbt_aux t2 \<rbrakk> \<Longrightarrow> is_rbt_aux (inter f t1 t2)"
   using rbt_sorted_inter rbt_inter
   by (auto simp: is_rbt_aux_prop)
 
@@ -1062,11 +1098,11 @@ lemma is_rbt_recolor: "is_rbt_aux t \<Longrightarrow> is_rbt (rbt_recolor t)"
 lemma is_rbt_dest: "is_rbt t \<Longrightarrow> is_rbt_aux t"
   by (auto simp: is_rbt_prop)
 
-lemma is_rbt_union: "is_rbt t1 \<Longrightarrow> is_rbt t2 \<Longrightarrow> is_rbt (rbt_recolor (union t1 t2))"
+lemma is_rbt_union: "is_rbt t1 \<Longrightarrow> is_rbt t2 \<Longrightarrow> is_rbt (rbt_recolor (union f t1 t2))"
   using is_rbt_aux_union
   by (auto dest!: is_rbt_dest intro: is_rbt_recolor)
 
-lemma is_rbt_inter: "is_rbt t1 \<Longrightarrow> is_rbt t2 \<Longrightarrow> is_rbt (rbt_recolor (inter t1 t2))"
+lemma is_rbt_inter: "is_rbt t1 \<Longrightarrow> is_rbt t2 \<Longrightarrow> is_rbt (rbt_recolor (inter f t1 t2))"
   using is_rbt_aux_inter
   by (auto dest!: is_rbt_dest intro: is_rbt_recolor)
 
@@ -1079,26 +1115,26 @@ end
 lemma is_rbt_union_comp:
   assumes "ID ccompare = Some (c :: ('a :: ccompare) comparator)"
     "ord.is_rbt (lt_of_comp c) t1" "ord.is_rbt (lt_of_comp c) t2"
-  shows "ord.is_rbt (lt_of_comp c) (rbt_recolor (union_comp c t1 t2))"
+  shows "ord.is_rbt (lt_of_comp c) (rbt_recolor (union_comp c f t1 t2))"
   using linorder.is_rbt_union[OF ID_ccompare[OF assms(1)] assms(2,3)]
     union_comp[OF ID_ccompare'[OF assms(1)]]
-  by auto
+  by metis
 
 lift_definition rbt_union_rbt_join2 :: "'a :: ccompare set_rbt \<Rightarrow> 'a set_rbt \<Rightarrow> 'a set_rbt" is
-  "\<lambda>t1 t2. rbt_recolor (union_comp ccomp t1 t2)"
+  "\<lambda>t1 t2. rbt_recolor (union_comp ccomp (\<lambda>_ _ _. ()) t1 t2)"
   using is_rbt_union_comp
   by force
 
 lemma is_rbt_inter_comp:
   assumes "ID ccompare = Some (c :: ('a :: ccompare) comparator)"
     "ord.is_rbt (lt_of_comp c) t1" "ord.is_rbt (lt_of_comp c) t2"
-  shows "ord.is_rbt (lt_of_comp c) (rbt_recolor (inter_comp c t1 t2))"
+  shows "ord.is_rbt (lt_of_comp c) (rbt_recolor (inter_comp c f t1 t2))"
   using linorder.is_rbt_inter[OF ID_ccompare[OF assms(1)] assms(2,3)]
     inter_comp[OF ID_ccompare'[OF assms(1)]]
-  by auto
+  by metis
 
 lift_definition rbt_inter_rbt_join2 :: "'a :: ccompare set_rbt \<Rightarrow> 'a set_rbt \<Rightarrow> 'a set_rbt" is
-  "\<lambda>t1 t2. rbt_recolor (inter_comp ccomp t1 t2)"
+  "\<lambda>t1 t2. rbt_recolor (inter_comp ccomp (\<lambda>_ _ _. ()) t1 t2)"
   using is_rbt_inter_comp
   by force
 
@@ -1108,7 +1144,7 @@ lemma is_rbt_minus_comp:
   shows "ord.is_rbt (lt_of_comp c) (rbt_recolor (minus_comp c t1 t2))"
   using linorder.is_rbt_minus[OF ID_ccompare[OF assms(1)] assms(2,3)]
     minus_comp[OF ID_ccompare'[OF assms(1)]]
-  by auto
+  by metis
 
 lift_definition rbt_minus_rbt_join2 :: "'a :: ccompare set_rbt \<Rightarrow> 'a set_rbt \<Rightarrow> 'a set_rbt" is
   "\<lambda>t1 t2. rbt_recolor (minus_comp ccomp t1 t2)"
@@ -1138,7 +1174,7 @@ proof (transfer)
     using assms
     by (auto simp: ord.is_rbt_def)
   show "set (RBT_Impl.keys t1) \<union> set (RBT_Impl.keys t2) =
-    set (RBT_Impl.keys (rbt_recolor (union_comp ccomp t1 t2)))"
+    set (RBT_Impl.keys (rbt_recolor (union_comp ccomp (\<lambda>_ _ _. ()) t1 t2)))"
     using linorder.rbt_sorted_union[OF ID_ccompare[OF id_ccomp] rbt_sorted_t]
     by (auto simp: union_comp[OF c])
 qed
@@ -1175,7 +1211,7 @@ proof (transfer)
     using assms
     by (auto simp: ord.is_rbt_def)
   show "set (RBT_Impl.keys t1) \<inter> set (RBT_Impl.keys t2) =
-    set (RBT_Impl.keys (rbt_recolor (inter_comp ccomp t1 t2)))"
+    set (RBT_Impl.keys (rbt_recolor (inter_comp ccomp (\<lambda>_ _ _. ()) t1 t2)))"
     using linorder.rbt_sorted_inter[OF ID_ccompare[OF id_ccomp] rbt_sorted_t1 rbt_sorted_t2]
     by (auto simp: inter_comp[OF c])
 qed
